proofs sequent & add_node + trilean + cleaning

yalla/mll.v
@@ -1,11 +1,11 @@
 (* Unit-free MLL following Yalla schemas *)
 
 
-From Coq Require Import Bool Wf_nat Lia.
+From Coq Require Import Bool Wf_nat.
 From OLlibs Require Import dectype funtheory List_more List_Type Permutation_Type_more.
 From mathcomp Require Import all_ssreflect zify.
 From GraphTheory Require Import preliminaries mgraph.
-(* check at the end if all are used *)
+(* TODO check at the end if all are used *)
 
 Import EqNotations.
 
@@ -125,7 +125,7 @@ Proof. destruct pi; cbn; by []. Qed.
 Lemma psize_rew l l' (pi : ll l) (Heq : l = l') : psize (rew Heq in pi) = psize pi.
 Proof. now subst. Qed.
 
-
+(* TODO cleaning above -> psize useless ? *)
 (*********************************************************************************************)
 (** ** Preliminaries *)
 
@@ -136,7 +136,7 @@ Proof.
   intros n i j ? ? H.
   assert (Hn : forall k : nat, k <= n -> nat_of_ord (@inord n k) = k).
   { intros. apply inordK. lia. }
-  by rewrite <-(Hn i), <-(Hn j), H.
+  by rewrite -(Hn i) // -(Hn j) // H.
 Qed.
 
 (** 'I_0 has the empty enumeration *)
@@ -153,8 +153,8 @@ Qed.
 Lemma case_I2bis : forall n : 'I_2, n = ord0 \/ n = ord1.
 Proof.
   intro n.
-  destruct (orP (case_I2 n)) as [H | H];
-  [left | right]; by apply /eqP.
+  assert (H := case_I2 n); revert H; move => /orP[/eqP H | /eqP H];
+  [by left | by right].
 Qed.
 
 Ltac destruct_I2 n H := destruct (case_I2bis n) as [H | H].
@@ -169,9 +169,8 @@ Qed.
 Lemma case_I3bis : forall n : 'I_3, n = ord0 \/ n = ord1 \/ n = ord2.
 Proof.
   intro n.
-  destruct (orP (case_I3 n)) as [H2 | H];
-  [destruct (orP H2) as [H | H]; clear H2| ];
-  [left | right; left | right; right]; by apply /eqP.
+  assert (H := case_I3 n); revert H; move => /orP[/orP[/eqP H | /eqP H] | /eqP H];
+  [by left | by right; left | by right; right].
 Qed.
 
 Ltac destruct_I3 n H := destruct (case_I3bis n) as [H | [H | H]].
@@ -184,25 +183,6 @@ Ltac destruct_I3 n H := destruct (case_I3bis n) as [H | [H | H]].
   under the form _ = _ or _ <> _, folding trivial cases *)
 Ltac case_if := repeat (let Hif := fresh "Hif" in
   case: ifP; cbn; move => /eqP Hif; rewrite ?Hif //).
-(* Ltac case2 := let Hif := fresh "Hif" in let Hif' := fresh "Hif" in
-case: ifP
-match goal with
-| H : ?x = ?x |- _ => assert (H = eq_refl) as ->
-                        by apply (Eqdep_dec.UIP_dec (@eq_dt_dec (list_dectype formulas_dectype)));
-                      cbn
-end. *)
-(* TODO generaliser case_if a ce test *)
-Lemma test (a b c : nat) : if ((a != b) || (b == c)) then true else false.
-Proof.
-case: ifP.
-(* match goal with
-| H : ?A || ?B |- _ => move => /orP H
-| H : (?A || ?B) = false |- _ => move => /norP H
-| H : ?a == ?b |- _ => move => /eqP H
-| H : ?a != ?b |- _ => move => /eqP H
-end. *)
-(* case_if. *)
-Admitted.
 
 
 (** * Type [rule] for the rule of a node *)
@@ -254,25 +234,6 @@ Ltac destruct_rule r H := destruct (case_rule r) as [[[[H | H] | H] | H] | H].
 (* TODO now useless ? *)
 (* TOTHINK rule as a finType ? possible if necessary *)
 
-(** * [comparison] is a DecType *)
-Definition eqb_comparison (A B : comparison) : bool :=
-  match A, B with
-  | Eq, Eq => true
-  | Lt, Lt => true
-  | Gt, Gt => true
-  | _, _ => false
-  end.
-
-Lemma eqb_eq_comparison : forall A B, eqb_comparison A B = true <-> A = B.
-Proof.
-  destruct A, B; split; cbn; intro H; trivial; now contradict H.
-Qed.
-
-Definition comparison_dectype := {|
-  car := comparison;
-  dectype.eqb := eqb_comparison;
-  eqb_eq := eqb_eq_comparison |}.
-
 
 (** * A DecType is an eqType *)
 Definition decType_eqMixin (X : DecType) := EqMixin (eq_dt_reflect (X:=X)).
@@ -282,9 +243,6 @@ Canonical formula_eqType := EqType formula (decType_eqMixin (formulas_dectype)).
 
 (* [rule] as an eqType *)
 Canonical rule_eqType := EqType rule (decType_eqMixin (rules_dectype)).
-
-(* [comparison] as an eqType *)
-Canonical comparison_eqType := EqType comparison (decType_eqMixin (comparison_dectype)).
 
 
 (** * Some results on cardinality *)
@@ -497,6 +455,27 @@ Proof.
 Qed.
 
 
+(** Lemma about pick *)
+Lemma p_pick_some (T : finType) (S : {set T}) (s : T) : [pick x in S] = Some s -> s \in S.
+Proof.
+  destruct (picksP S); try by [].
+  move => /eqP H; revert H; cbn; move => /eqP H; by rewrite -H.
+Qed.
+
+Lemma p_pick_none (T : finType) (S : {set T}) : [pick x in S] = None -> #|S| = 0.
+Proof.
+  destruct (picksP S); try by [].
+  subst; by rewrite cards0.
+Qed.
+
+
+(** Set with 3 elements for case tens, parr and cut *)
+Inductive trilean :=
+  | tens_t
+  | parr_t
+  | cut_t.
+
+
 
 (** ** Level 0: Multigraphs from the library GraphTheory *)
 (** * Notations from the library *)
@@ -512,11 +491,6 @@ Definition edges_at_subset (b : bool) {Lv : Type} {Le : Type} {G : graph Lv Le} 
 Notation edges_out_at_subset := (edges_at_subset false).
 Notation edges_in_at_subset := (edges_at_subset true).
 
-Definition edges_out_at_set {Lv : Type} {Le : Type} {G : graph Lv Le} (v : G) : finType :=
-  [finType of {e : edge G | source e == v}].
-Definition edges_in_at_set {Lv : Type} {Le : Type} {G : graph Lv Le} (v : G) : finType :=
-  [finType of {e : edge G | target e == v}].
-
 
 
 (** ** Level 1: Multigraphs with some more data *)
@@ -530,49 +504,16 @@ Record graph_data : Type :=
   }.
 Unset Primitive Projections.
 
-(* sig [eta mem S] avec S : {set G} *)
-(* idées:
-- direction avec type totaux (directement sur vertex -> edges)
-- sum type pour avoir toutes les informations et contraintes selon le type de noeuds,
-  codé en tant que 
-- ajouter une donnée n et order = fonction de I_n vers des neouds/aretes ;
-    ou une liste de noeuds/aretes, sans le n
-- definir juste left, en deduire right apres
-- curryfier les sigma input
-
-TOTHINK other possibilities for the functions:
-    order : [concl_l node] -> 'I_#|concl_l node]|;
-avec    order_inj : injective order;
-
-    order : {perm {v : graph_of | vlabel v == concl_l}};
-  -     direction : bool -> vertex graph_of -> edge graph_of; avec
-Notation left := (direction false).
-Notation right := (direction true).
-  -> {v : graph_of | (vlabel v == tens_l) || (vlabel v == parr_l)}
-  - faire des fonctions depuis les ensembles totaux vers option _ puis lemma
-    pour label ok <-> Some _
-    ex:
-      order : graph_of -> option nat;
-      order_ok : forall v, exists n, order v = Some n <-> vlabel v = concl_l /\
-            order v <= nb nodes concl;
-          en fait si injectif, pas necessaire d'avoir la dernière condition,
-          qui semble etre la plus difficile comme #|_| est dur à calculer
-      direction : bool -> graph_of -> option_finType (edge graph_of);
-      direction_ok : forall b v, direction b v = Some _ <->
-          (vlabel c = tens_l \/ vlabel c = parr_l);
-  - see sig_finType, used for the function sub_edge in the graph lib
-  - other way to define bijections for order: surj instead of inj, from I_n -> vertices, ...
-  - something else ?
-  - define order as a permutation of the finset as finset = seq = list, easier to manipulate
-      --> NON
-  - dans direction, restreindre edge to edge_in_at_set v ?
-  - mettre direction et ordre plutot dans proof_structure ? (ie cette couche est inutile ?)
+(* TOTHINK
+  - direction : bool -> vertex graph_of -> edge graph_of; Notation left := (direction false).
+  - faire des fonctions depuis les ensembles totaux vers option _ puis lemma pour label ok <-> Some _
+    ex: direction : bool -> graph_of -> option_finType (edge graph_of);
+        direction_ok : forall b v, direction b v = Some _ <-> (vlabel c = tens_l \/ vlabel c = parr_l);
+  - see sig_finType, used for the function sub_edge in the graph lib : sig [eta mem S] avec S : {set G}
+  - sum type pour avoir toutes les informations et contraintes selon le type de noeuds, codé en tant que 
+  - mettre direction et ordre plutot dans proof_structure ? (ie cette couche est inutile ?) something else ?
 *)
-
-(* fonction qui dit si formule atomique existe dans yalla,
-  possible de l'ajouter pour expansion atome *)
-(* /!\ faire lemma (admitted dependant des defs), pour utiliser
-  independamment de la def choisie *)
+(* TOTHINK fonction qui dit si formule atomique existe dans yalla, possible de l'ajouter pour expansion atome *)
 
 (** * Functions to weaken a proof *)
 Lemma tens_to_tensparr : forall (l : rule), l = tens_l -> l = tens_l \/ l = parr_l.
@@ -606,12 +547,11 @@ Definition ax_graph (x : atom) : graph rule formula := {|
      O     <--------    O   ------->   O
     ord1      ord0    ord0    ord1    ord2   *)
 
-Definition ax_left (x : atom) : vertex (ax_graph x) -> edge (ax_graph x) :=
-  fun _ => ord0. (* no vertex tens nor parr: we put a nonsensical value *)
+Definition ax_left (x : atom) : vertex (ax_graph x) -> edge (ax_graph x) := fun _ => ord0.
+(* No vertex tens nor parr: nonsensical value *)
 Arguments ax_left : clear implicits.
 
-Definition ax_order (x : atom) : list (vertex (ax_graph x)) :=
-  ord1 :: ord2 :: nil.
+Definition ax_order (x : atom) : list (vertex (ax_graph x)) := ord1 :: ord2 :: nil.
 
 Definition ax_graph_data (x : atom) : graph_data := {|
   graph_of := ax_graph x;
@@ -632,12 +572,10 @@ Definition union_left (G0 G1 : graph_data) : G0 ⊎ G1 -> edge (G0 ⊎ G1) :=
 Arguments union_left : clear implicits.
 
 (** Function order for a disjoint union *)
-(* Put the two first premises at the beginning, then the tail of order G1,
-   finally the tail of order G0 *)
+(* Put the two first premises at the beginning, then the tail of order G1, finally the tail of order G0 *)
 Definition union_order (G0 G1 : graph_data) : list (G0 ⊎ G1) :=
   match order G0, order G1 with
   | v0 :: o0, v1 :: o1 => inl v0 :: inr v1 :: map inr o1 ++ map inl o0
-(* but order will never be nil, so other cases not encountered *)
   | _, [::] => map inl (order G0)
   | [::], _ => map inr (order G1)
   end.
@@ -672,8 +610,7 @@ Proof.
   intros [e | e].
   all: assert (Hfe: injective fe) by (apply inl_inj || apply inr_inj).
   all: rewrite ?inj_imset // !in_set; cbn; trivial.
-  all: apply /eqP /memPn.
-  all: move => y /imsetP [? _] Hl.
+  all: apply /eqP /memPn; move => y /imsetP [? _] Hl.
   all: by rewrite Hl.
 Qed.
 Notation union_edges_at_inl := (union_edges_at (i := false)).
@@ -710,109 +647,94 @@ Qed.
 Notation union_order_inl := (union_order_in (i := false)).
 Notation union_order_inr := (union_order_in (i := true)).
 
-(* BUG REPORT
+(* TODO BUG REPORT *)
 (* c'est bien long à compiler ... mais ça ne l'est pas sans les let des noms de sommets !? *)
-(* isoler le probleme, montrer exponentiel en temps selon le nombre de inl,
-   puis faire un bug report *)
-Definition add_parr_quick {G : graph_data} (e0 e1 : edge G) :=
-  (* add new vertices parr and concl *)
-  let G1 := (G ∔ parr_l) ∔ concl_l in
-  (* duplicate edges e0 and e1 to parr, from s0 and s1, and add an edge from parr to concl *)
+(* isoler le probleme, montrer exponentiel en temps selon le nombre de inl, puis faire un bug report *)
+(*
+Definition add_parr_quick {Lv Le : Type} (a b : Lv) {G : graph Lv Le} (e0 e1 : edge G) :=
+  let G1 := (G ∔ a) ∔ b in
   let G2 := G1 ∔ [ inl (inl (source e0)) , elabel e0 , inl (inr tt) ]
-    ∔ [ inl (inl (source e1)) , elabel e1 , inl (inr tt) ]
-    ∔ [ inl (inr tt) , parr (elabel e0) (elabel e1) , inr tt ] in
-  (* remove t0 and t1 *)
+               ∔ [ inl (inl (source e1)) , elabel e1 , inl (inr tt) ]
+               ∔ [ inl (inr tt) , elabel e0 , inr tt ] in
   let S : {set G2} := setT :\ inl (inl (target e0)) :\ inl (inl (target e1)) in
   induced S.
-Definition add_parr_slow {G : graph_data} (e0 e1 : edge G) :=
-  (* add new vertices parr and concl *)
-  let G1 := (G ∔ parr_l) ∔ concl_l in
+Definition add_parr_slow {Lv Le : Type} (a b : Lv) {G : graph Lv Le} (e0 e1 : edge G) :=
+  let G1 := (G ∔ a) ∔ b in
   let s0 := inl (inl (source e0)) : G1 in
   let t0 := inl (inl (target e0)) : G1 in
   let s1 := inl (inl (source e1)) : G1 in
   let t1 := inl (inl (target e1)) : G1 in
   let v_parr := inl (inr tt) : G1 in
   let v_concl := inr tt : G1 in
-  (* duplicate edges e0 and e1 to parr, from s0 and s1, and add an edge from parr to concl *)
   let G2 := G1 ∔ [ s0 , elabel e0 , v_parr ]
-    ∔ [ s1 , elabel e1 , v_parr ]
-    ∔ [ v_parr , parr (elabel e0) (elabel e1) , v_concl ] in
-  (* remove t0 and t1 *)
-  let S : {set G2} := [set x | (x != t0) && (x != t1)] in
+               ∔ [ s1 , elabel e1 , v_parr ]
+               ∔ [ v_parr , elabel e0, v_concl ] in
+  let S : {set G2} := setT :\ inl (inl (target e0)) :\ inl (inl (target e1)) in
   induced S.
 *)
 
 (** * Adding a node to a graph_data *)
 (** Add a tens/parr/cut node to a graph_data, replacing 2 conclusions *)
 (* Add a tens/parr/cut node, without removing conclusions *)
-Definition add_node_graph_1 (c : comparison) {G : graph_data} (e0 e1 : edge G) :=
+Definition add_node_graph_1 (c : trilean) {G : graph_data} (e0 e1 : edge G) :=
   (* subgraph to add *)
-  let graph_node (b : comparison) := match b with
-    | Eq => edge_graph tens_l (tens (elabel e0) (elabel e1)) concl_l
-    | Lt => edge_graph parr_l (parr (elabel e0) (elabel e1)) concl_l
-    | Gt => unit_graph cut_l
+  let graph_node (b : trilean) := match b with
+    | tens_t => edge_graph tens_l (tens (elabel e0) (elabel e1)) concl_l
+    | parr_t => edge_graph parr_l (parr (elabel e0) (elabel e1)) concl_l
+    | cut_t => unit_graph cut_l
   end in
-  let G1 (b : comparison) := G ⊎ graph_node b in
+  let G1 (b : trilean) := G ⊎ graph_node b in
   (* node of the graph receving edges *)
   let target_node := match c return G1 c with
-    | Eq => inr (inl tt)
-    | Lt => inr (inl tt)
-    | Gt => inr tt
+    | tens_t => inr (inl tt)
+    | parr_t => inr (inl tt)
+    | cut_t => inr tt
   end in
   (* duplicate edges *)
   G1 c ∔ [ inl (source e0) , elabel e0 , target_node ]
        ∔ [ inl (source e1) , elabel e1 , target_node ].
 
 (* Remove the conclusions *)
-Definition add_node_graph (c : comparison) {G : graph_data} (e0 e1 : edge G) :=
+Definition add_node_graph (c : trilean) {G : graph_data} (e0 e1 : edge G) :=
   let G' := add_node_graph_1 c e0 e1 in
   let S : {set G'} := setT :\ inl (target e0) :\ inl (target e1) in
   induced S.
 
 (** Function left for the graph with a new node *)
 (* Function left for the intermediary graph *)
-Definition add_node_left_1 (c : comparison) {G : graph_data} (e0 e1 : edge G) :=
+Definition add_node_left_1 (c : trilean) {G : graph_data} (e0 e1 : edge G) :=
   let G' := add_node_graph_1 c e0 e1 in
   fun (v : G') => match v return edge G' with
-  | inl u => (* if (target (left u) != target e1) && (target (left u) != target e0)
-    then Some (Some (inl (left u)))
-    else Some None *)
-            if target (left u) == target e0 then Some None
-            else if target (left u) == target e1 then Some None
-            else Some (Some (inl (left u)))
+  | inl u => if target (left u) == target e0 then Some None
+             else if target (left u) == target e1 then Some None
+             else Some (Some (inl (left u)))
 (* artefact for when the value of left is nonsensical:
-if target left v is the c node we remove (ie if we remove the edge left v),
-we have to give it a new value in the updated left;
-in this case, left v is the (unique input) edge of a c node,
-so not the input edge of a tens or a parr, we can give it any value *)
+if target (left v) is the node we remove, we have to give a new (nonsensial) value for the new left *)
   | inr _ => Some None
   end.
-(* TOTHINK Damien Pous possible de simplifier ce if / faire autrement ? *)
-(* ajouter conditions (source (left u) != target e0 &&
-  source (left u) != target e1) dans le if ? *)
-(* TOTEST left avec option, pour eviter ce if + ajouter un invariant dans geos
-pour target (left v) = Some v si v est un tens / parr *)
+(* TOTHINK Damien Pous possible de simplifier ce if / faire autrement ?
+   ajouter conditions (source (left u) != target e0 && source (left u) != target e1) dans le if ? *)
+(* TOTEST left avec option, pour eviter ce if + ajouter un invariant dans geos pour target (left v) = Some v si v est un tens / parr *)
 
 (* Necessary hypothesis : the nodes we remove have no input edges *)
-Lemma add_node_consistent_left (c : comparison) {G : graph_data} (e0 e1 : edge G) :
+Lemma add_node_consistent_left (c : trilean) {G : graph_data} (e0 e1 : edge G) :
   let G' := add_node_graph_1 c e0 e1 in
   let S : {set G'} := setT :\ inl (target e0) :\ inl (target e1) in
-  (forall e, source e != target e0) -> (forall e, source e != target e1) ->
+  (forall e, source e != target e0) /\ (forall e, source e != target e1) ->
   forall v : G', add_node_left_1 v \in edge_set S.
 Proof.
   destruct c; cbn;
-  intros H0 H1 [v | v];
+  intros [H0 H1] [v | v];
   rewrite !in_set; cbn;
   repeat (apply /andP; split); trivial.
   all: case_if; by apply/eqP.
 Qed.
 
 (* Function left for the graph with a new node *)
-Definition add_node_left (c : comparison) {G : graph_data} (e0 e1 : edge G)
-  (H0 : forall e : edge G, source e != target e0)
-  (H1 : forall e : edge G, source e != target e1) :
+Definition add_node_left (c : trilean) {G : graph_data} (e0 e1 : edge G)
+  (H : (forall e : edge G, source e != target e0) /\ (forall e : edge G, source e != target e1)) :
   add_node_graph c e0 e1 -> edge (add_node_graph c e0 e1) :=
-  fun v => Sub (add_node_left_1 (val v)) (add_node_consistent_left H0 H1 (val v)).
+  fun v => Sub (add_node_left_1 (val v)) (add_node_consistent_left H (val v)).
 
 (** Function order for the graph with a new node *)
 (* Remove the 2 nodes from order *)
@@ -820,18 +742,17 @@ Definition add_node_order_1 {G : graph_data} (e0 e1 : edge G) :=
   [seq x <- order G | (x != target e0) && (x != target e1)].
 
 (* Give order the type of the intermediary graph *)
-Definition add_node_type_order (c : comparison) {G : graph_data} (e0 e1 : edge G)
-  (l : list G) : list (add_node_graph_1 c e0 e1) :=
-  [seq (inl v) | v <- l].
+Definition add_node_type_order (c : trilean) {G : graph_data} (e0 e1 : edge G) (l : list G) :
+  list (add_node_graph_1 c e0 e1) := [seq (inl v) | v <- l].
 
 (* Add the new conclusion if it exists *)
-Definition add_node_order_2 (c : comparison) {G : graph_data} (e0 e1 : edge G) :=
+Definition add_node_order_2 (c : trilean) {G : graph_data} (e0 e1 : edge G) :=
   match c return list (add_node_graph_1 c e0 e1) with
-  | Eq as c | Lt as c => inr (inr tt) :: add_node_type_order c e0 e1 (add_node_order_1 e0 e1)
-  | Gt as c => add_node_type_order c e0 e1 (add_node_order_1 e0 e1)
+  | tens_t as c | parr_t as c => inr (inr tt) :: add_node_type_order c e0 e1 (add_node_order_1 e0 e1)
+  | cut_t as c => add_node_type_order c e0 e1 (add_node_order_1 e0 e1)
   end.
 
-Lemma add_node_consistent_order (c : comparison) {G : graph_data} (e0 e1 : edge G) :
+Lemma add_node_consistent_order (c : trilean) {G : graph_data} (e0 e1 : edge G) :
   let G' := add_node_graph_1 c e0 e1 in
   let S : {set G'} := setT :\ inl (target e0) :\ inl (target e1) in
   all (pred_of_set S) (add_node_order_2 c e0 e1).
@@ -848,16 +769,16 @@ Proof.
   by apply (in_notin (l := add_node_order_2 c e0 e1)).
 Qed.
 
-Definition add_node_order (c : comparison) {G : graph_data} (e0 e1 : edge G) :
+Definition add_node_order (c : trilean) {G : graph_data} (e0 e1 : edge G) :
   list (vertex (add_node_graph c e0 e1)) :=
-  [seq v | v <- sval (all_sigP (add_node_consistent_order c e0 e1))].
+  sval (all_sigP (add_node_consistent_order c e0 e1)).
 
 (** Graph data for adding a node *)
-Definition add_node_graph_data (c : comparison) {G : graph_data} (e0 e1 : edge G)
-  (H0 : forall e : edge G, source e != target e0)
-  (H1 : forall e : edge G, source e != target e1) : graph_data := {|
+Definition add_node_graph_data (c : trilean) {G : graph_data} (e0 e1 : edge G)
+  (H : (forall e : edge G, source e != target e0) /\ (forall e : edge G, source e != target e1)) :
+  graph_data := {|
   graph_of := add_node_graph c e0 e1;
-  left := add_node_left H0 H1;
+  left := add_node_left H;
   order := add_node_order c e0 e1;
   |}.
 
@@ -885,8 +806,7 @@ Definition deg (b : bool) := match b with
 Notation deg_out := (deg false).
 Notation deg_in := (deg true).
 
-(* TODO see if proper in bool needed later on and
-if edeges_in_at_subset or edges_in_at_set better *)
+(* TODO see if proper in bool needed later on *)
 (** Property of a geometric structure *)
 Definition proper_degree (G : graph_data) :=
   forall (b : bool) (v : G), #|edges_at_subset b v| = deg b (vlabel v).
@@ -913,12 +833,21 @@ Notation p_deg_in := (p_deg true).
 
 (** * Derivated results on a geometric structure *)
 (* Nonsensical values for total functions on vertices but where only some vertices matters *)
-Definition bogus {G : geos} (v : G) : edge G := left v.
+Definition bogus {G : graph_data} : G -> edge G := fun v => left v.
+
+Lemma p_left3 (G : geos) :
+  forall (v : G), vlabel v = tens_l \/ vlabel v = parr_l ->
+  target (left v) = v.
+Proof.
+  intros v Hv.
+  assert (H := p_left Hv).
+  rewrite in_set in H; by apply /eqP.
+Qed.
 
 (** Function right for the right premisse of a tens / parr *)
 Lemma unique_right (G : geos) :
   forall (v : G), vlabel v = tens_l \/ vlabel v = parr_l -> #|edges_in_at_subset v| = 2.
-Proof. intros v [Hl | Hl]; by rewrite (p_deg_in v) Hl. Qed.
+Proof. intros v [Hl | Hl]; by rewrite p_deg Hl. Qed.
 
 Definition right : forall G : geos, G -> edge G :=
   fun (G : geos) (v : G) =>
@@ -931,7 +860,7 @@ Definition right : forall G : geos, G -> edge G :=
     other (unique_right H') (p_left H')
   | _ => fun _ => bogus v
   end Logic.eq_refl.
-
+(* TODO better name for these properties *)
 Lemma p_right (G : geos) :
   forall (v : G), vlabel v = tens_l \/ vlabel v = parr_l ->
   right v \in edges_in_at_subset v /\ right v != left v.
@@ -965,24 +894,23 @@ Proof.
   all: apply p_other2.
 Qed.
 
-(* debut modif *)
-(* 3e possibilite: mettre right et ccl comme left + proper à la place des lemmes deduisibles *)
+Lemma p_right3 (G : geos) :
+  forall (v : G), vlabel v = tens_l \/ vlabel v = parr_l ->
+  target (right v) = v.
+Proof.
+  intros v Hv.
+  assert (H := p_right Hv).
+  revert H; rewrite in_set; by move => [/eqP H _].
+Qed.
+
+(* General right *)
 Definition right' : forall G : graph_data, G -> edge G :=
   fun G (v : G) => 
   match [pick x in (edges_in_at_subset v) :\ left v] with
   | Some e => e
-  | None => left v
+  | None => bogus v
   end.
-Lemma p_pick_some (T : finType) (S : {set T}) (s : T) : [pick x in S] = Some s -> s \in S.
-Proof.
-  destruct (picksP S); try by [].
-  move => /eqP H; revert H; cbn; move => /eqP H; by rewrite -H.
-Qed.
-Lemma p_pick_none (T : finType) (S : {set T}) : [pick x in S] = None -> #|S| = 0.
-Proof.
-  destruct (picksP S); try by [].
-  subst; by rewrite cards0.
-Qed.
+
 Lemma right_eq (G : geos) : forall (v : G), vlabel v = tens_l \/ vlabel v = parr_l ->
   right v = right' v.
 Proof.
@@ -1001,14 +929,13 @@ Proof.
     destruct Hv as [Hv | Hv];
     by rewrite Hv.
 Qed.
-(* fin modif *)
 
 
 (** Function ccl for the conclusion of a tens / parr *)
 Lemma unique_ccl (G : geos) :
   forall (v : G), vlabel v = tens_l \/ vlabel v = parr_l ->
   #|edges_out_at_subset v| = 1.
-Proof. intros v [Hl | Hl]; by rewrite (p_deg_out v) Hl. Qed.
+Proof. intros v [Hl | Hl]; by rewrite p_deg Hl. Qed.
 
 Definition ccl : forall G : geos, G -> edge G :=
   fun (G : geos) (v : G) =>
@@ -1052,14 +979,23 @@ Proof.
   all: apply p_pick_unique.
 Qed.
 
-(* debut modif *)
-(* 3e possibilite: mettre right et ccl comme left + proper à la place des lemmes deduisibles *)
+Lemma p_ccl3 (G : geos) :
+  forall (v : G), vlabel v = tens_l \/ vlabel v = parr_l ->
+  source (ccl v) = v.
+Proof.
+  intros v Hv.
+  assert (H := p_ccl Hv).
+  rewrite in_set in H; by apply /eqP.
+Qed.
+
+(* General ccl *)
 Definition ccl' : forall G : graph_data, G -> edge G :=
-  fun G (v : G) => 
+  fun G (v : G) =>
   match [pick x in (edges_out_at_subset v)] with
   | Some e => e
-  | None => left v
+  | None => bogus v
   end.
+
 Lemma ccl_eq (G : geos) : forall (v : G), vlabel v = tens_l \/ vlabel v = parr_l ->
   ccl v = ccl' v.
 Proof.
@@ -1075,14 +1011,13 @@ Proof.
     destruct Hv as [Hv | Hv];
     by rewrite Hv.
 Qed.
-(* fin modif *)
 
 
 (** Function returning the unique (input) edge of a conclusion *)
 Lemma unique_concl (G : geos) :
   forall (v : G), vlabel v = concl_l ->
   #|edges_in_at_subset v| = 1.
-Proof. intros v Hl; by rewrite (p_deg_in v) Hl. Qed.
+Proof. intros v Hl; by rewrite p_deg Hl. Qed.
 
 Definition edge_of_concl : forall G : geos, G -> edge G :=
   fun (G : geos) (v : G) =>
@@ -1127,10 +1062,33 @@ Lemma p_concl3 (G : geos) :
   target (edge_of_concl v) = v.
 Proof.
   intros v Hv.
-  assert (H : edge_of_concl v \in edges_in_at_subset v) by by apply p_concl.
-  rewrite in_set in H.
-  by apply /eqP.
+  assert (H := p_concl Hv).
+  rewrite in_set in H; by apply /eqP.
 Qed.
+
+(* General edge_of_concl *)
+Definition edge_of_concl' : forall G : graph_data, G -> edge G :=
+  fun G (v : G) => 
+  match [pick x in (edges_in_at_subset v)] with
+  | Some e => e
+  | None => bogus v
+  end.
+
+Lemma edge_of_concl_eq (G : geos) : forall (v : G), vlabel v = concl_l ->
+  edge_of_concl v = edge_of_concl' v.
+Proof.
+  intros v Hv.
+  unfold edge_of_concl'.
+  all: destruct ([pick x in edges_in_at_subset v]) as [e | ] eqn:He.
+  - assert (Hin := p_pick_some He).
+    revert Hin.
+    rewrite p_concl2 // !in_set.
+    by move => /eqP H.
+  - assert (H0 := p_pick_none He).
+    contradict H0.
+    by rewrite p_deg Hv.
+Qed.
+
 
 (** Sequent proved by the proof structure *)
 Definition sequent (G : geos) : list formula :=
@@ -1183,9 +1141,6 @@ Definition ax_geos (x : atom) : geos := {|
   p_left := ax_p_left x;
   p_order := ax_p_order x;
   |}.
-
-Lemma ax_nb_concl (x : atom) : #|[set v : ax_graph_data x | vlabel v == concl_l]| = 2.
-Proof. compute_card_subIn. Qed. (* useless ? *)
 
 
 (** * A disjoint union of geos is a geos *)
@@ -1311,27 +1266,14 @@ Proof.
   all: assert (Hout : edges_out_at_subset v = set0) by (apply cards0_eq; by rewrite (p_deg_out v) Hv).
   all: by rewrite -(in_set0 e) -Hout in_set.
 Qed.
-Definition add_node_hyp0 (G : geos) (v0 v1 : G) (l : seq G) (H : order G = v0 :: v1 :: l) :
-forall e : edge G, source e != target (edge_of_concl v0).
-Proof. apply (add_node_hyp H). Defined.
-Definition add_node_hyp1 (G : geos) (v0 v1 : G) (l : seq G) (H : order G = v0 :: v1 :: l) :
-forall e : edge G, source e != target (edge_of_concl v1).
-Proof. apply (add_node_hyp H). Defined.
 
-Definition add_node_graph_data_bis : comparison -> geos -> graph_data :=
-  fun (c : comparison) (G : geos) =>
-  match order G as o return order G = o -> graph_data with
-  | _ :: _ :: _ => fun Heq => add_node_graph_data c (add_node_hyp0 Heq) (add_node_hyp1 Heq)
-  | _ => fun _ => G (* do nothing if there is not at least 2 nodes conclusion *)
-end Logic.eq_refl.
-
-Definition add_node_transport_1 (c : comparison) (G : graph_data) (e0 e1 : edge G) :
+Definition add_node_transport_1 (c : trilean) (G : graph_data) (e0 e1 : edge G) :
   edge G -> edge (add_node_graph_1 c e0 e1) :=
   fun e => if (e == e1) then None
            else if (e == e0) then Some None
            else Some (Some (inl e)).
 
-Lemma add_node_transport_consistent (c : comparison) (G : geos) (v0 v1 : G) (l : seq G)
+Lemma add_node_transport_consistent (c : trilean) (G : geos) (v0 v1 : G) (l : seq G)
   (H : order G = v0 :: v1 :: l) :
   forall e, add_node_transport_1 c (edge_of_concl v0) (edge_of_concl v1) e \in
   edge_set (setT :\ inl (target (edge_of_concl v0)) :\ inl (target (edge_of_concl v1)) :
@@ -1343,18 +1285,17 @@ Proof.
     rewrite H !in_cons eq_refl //.
     apply /orP; by right. }
   set e0 := edge_of_concl v0; set e1 := edge_of_concl v1.
-  destruct (add_node_hyp H) as [H0 H1].
   set S := setT :\ inl (target e0) :\ inl (target e1) : {set add_node_graph_1 c e0 e1}.
   assert (None \in edge_set S /\ Some None \in edge_set S) as [Hn Hsn].
   { rewrite !in_set.
     split; repeat (apply /andP; split); trivial;
-    try (apply H0 || apply H1);
+    try apply (add_node_hyp H);
     rewrite p_concl3 //; by destruct c. }
   intro e.
   unfold add_node_transport_1; case_if.
   rewrite !in_set.
   repeat (apply /andP; split); trivial.
-  1:{ apply H1. } 1:{ apply H0. }
+  1,2: apply (add_node_hyp H).
   all: rewrite p_concl3 //.
   all: apply /negP; intro.
   1: set et := e1. 2: set et := e0.
@@ -1362,149 +1303,13 @@ Proof.
   all: by contradict Hc.
 Qed.
 
-Definition add_node_transport (c : comparison) (G : geos) (v0 v1 : G) (l : seq G)
+Definition add_node_transport (c : trilean) (G : geos) (v0 v1 : G) (l : seq G)
   (H : order G = v0 :: v1 :: l) :
-  edge G -> edge (add_node_graph_data c (add_node_hyp0 H) (add_node_hyp1 H)) :=
+  edge G -> edge (add_node_graph_data c (add_node_hyp H)) :=
   fun e => Sub (add_node_transport_1 c (edge_of_concl v0) (edge_of_concl v1) e)
     (add_node_transport_consistent c H e).
-(* TODO modifier lemma avec : *)
-Definition add_node_transport' (c : comparison) (G : geos) : edge G -> edge (add_node_graph_data_bis c G).
-Proof.
-  unfold add_node_graph_data_bis.
-  generalize (erefl (order G));
-  destruct (order G) as [ | v0 [ | v1 l]] at 2 3;
-  intro H.
-  - apply id.
-  - apply id.
-  - apply (fun e => Sub (add_node_transport_1 c (edge_of_concl v0) (edge_of_concl v1) e)
-      (add_node_transport_consistent c H e)).
-Defined.
 
-Definition g (c : comparison) (G : geos) : edge (add_node_graph_data_bis c G) -> edge G.
-Proof.
-  unfold add_node_graph_data_bis.
-  generalize (erefl (order G));
-  destruct (order G) as [ | v0 [ | v1 l]] at 2 3;
-  intro H.
-  - apply id.
-  - apply id.
-  - intros [[[[e | e] | ] | ] He].
-    + apply e.
-    + apply (edge_of_concl v0).
-    + apply (edge_of_concl v0).
-    + apply (edge_of_concl v1).
-Defined. (* pour injective' *)
-Lemma add_node_transport_inj' (c : comparison) (G : geos) :
-  injective (add_node_transport' c (G := G)).
-Proof.
-  apply (can_inj (g := @g c G)).
-  unfold cancel, add_node_transport', g.
-  intro e.
-  generalize (erefl (order G)).
-  destruct (order G) as [ | v0 [ | v1 l]] at 2 3 17;
-  trivial.
-  intro H.
-  destruct (Sub (add_node_transport_1 c (edge_of_concl v0) (edge_of_concl v1) e)
-     (add_node_transport_consistent c H e)) as [[[[f | f] | ] | ] Hf] eqn:Hef;
-  assert (Hef' := EqdepFacts.eq_sig_fst Hef).
-  all: revert Hef'; unfold add_node_transport_1; case_if.
-  by move => /eqP Hef'; cbn in Hef'; revert Hef'; move => /eqP Hef'.
-Qed. Print add_node_graph_1.
-Definition add_node_transport_v_1 (c : comparison) (G : graph_data) (e0 e1 : edge G) :
-  G -> add_node_graph_1 c e0 e1 :=
-  let t := match c as b return (add_node_graph_1 b e0 e1) with
-    | Gt => inr tt
-    | _ => inr (inl tt)
-    end in
-  fun v => if (v == target e1) then t
-           else if (v == target e0) then t
-           else inl v.
-Lemma add_node_transport_v_consistent (c : comparison) (G : geos) (v0 v1 : G) (l : seq G)
-  (H : order G = v0 :: v1 :: l) :
-  forall v, add_node_transport_v_1 c (edge_of_concl v0) (edge_of_concl v1) v \in
-  (setT :\ inl (target (edge_of_concl v0)) :\ inl (target (edge_of_concl v1)) :
-  {set add_node_graph_1 c (edge_of_concl v0) (edge_of_concl v1)}).
-Proof.
-  set e0 := edge_of_concl v0; set e1 := edge_of_concl v1.
-  set S := setT :\ inl (target e0) :\ inl (target e1) : {set add_node_graph_1 c e0 e1}.
-  intro v.
-  unfold add_node_transport_v_1; case_if;
-  rewrite !in_set.
-  all: try by destruct c.
-  repeat (apply /andP; split); cbn; by apply /eqP.
-Qed.
-(* TODO modifier lemma avec : *)
-Definition add_node_transport_v (c : comparison) (G : geos) : G -> add_node_graph_data_bis c G.
-Proof.
-  unfold add_node_graph_data_bis.
-  generalize (erefl (order G));
-  destruct (order G) as [ | v0 [ | v1 l]] at 2 3;
-  intro H.
-  - apply id.
-  - apply id.
-  - apply (fun v => Sub (add_node_transport_v_1 c (edge_of_concl v0) (edge_of_concl v1) v)
-      (add_node_transport_v_consistent c H v)).
-Defined.
-Lemma add_node_transport_edges' (c : comparison) (G : geos) :
-  forall (v : G) (b : bool),
-  edges_at_subset b (add_node_transport_v c v) =
-  [set add_node_transport' c e | e in edges_at_subset b v].
-(* FAUX si v = target e0 ou target e1 *)
-Proof.
-  unfold add_node_graph_data_bis, add_node_transport_v, add_node_transport'.
-  generalize (erefl (order G)).
-  destruct (order G) as [ | v0 [ | v1 l]] at 2 3 9 15 21 35 41;
-  intros H v b;
-  try (by rewrite imset_id).
-  assert (vlabel v0 = concl_l /\ vlabel v1 = concl_l) as [Hv0  Hv1].
-  { destruct (p_order G) as [O _].
-    split; apply O;
-    rewrite H !in_cons eq_refl //.
-    apply /orP; by right. }
-  set e0 := edge_of_concl v0; set e1 := edge_of_concl v1.
-  assert (Hneqv : v0 != v1).
-  { elim (p_order G).
-    rewrite H cons_uniq in_cons negb_or.
-    by move => _ /andP[/andP[? _] _]. }
-  assert (Hneqe : e0 == e1 = false).
-  { apply negbTE, (contra_neq (z1 := target e0) (z2 := target e1)).
-    - apply f_equal.
-    - by rewrite !p_concl3. }
-  apply /setP; intro e.
-  assert (Hv := add_node_transport_v_consistent c H v).
-  set g_1 := add_node_transport_1 c e0 e1.
-  set g := fun e2 => Sub (add_node_transport_1 c e0 e1 e2) (add_node_transport_consistent c H e2).
-assert (injective g).
-{ unfold g. intros x y H'. assert(H'':= EqdepFacts.eq_sig_fst H').
-revert H''. unfold add_node_transport_1. case_if. move => /eqP H''; by apply /eqP. }
-  set g_inj := add_node_transport_inj' (c:=c) (G:=G).
-  destruct e as [[[[e | e] | ] | ] He];
-  rewrite in_set; cbn; rewrite !SubK; cbn.
-  - assert (Heq : Sub (Some (Some (inl e))) He = g e).
-    { apply /eqP; rewrite /g /add_node_transport sub_val_eq SubK /add_node_transport_1.
-      case_if.
-      all: contradict He.
-      all: rewrite ?Hif ?Hif0 !in_set.
-      1: move => /andP[_ /andP[He _]].
-      2: move => /andP[_ /andP[_ /andP[He _]]].
-      all: contradict He; apply /negP; by rewrite negb_involutive. }
-    rewrite Heq inj_imset // in_set /add_node_transport_v_1.
-    clear Heq; revert He; rewrite !in_set; cbn;
-    move => /andP[/andP[? /andP[? _]] /andP[? /andP[? _]]].
-    case_if; destruct c, b; cbn; symmetry; by apply /eqP /eqP.
-  - assert (Hin : Sub (Some (Some (inr e))) He \in [set g x | x in edges_at_subset b v] = false).
-    { apply /negbTE.
-      rewrite Imset.imsetE in_set.
-      apply /imageP; move => [a _ A].
-      assert (Hc : Some (Some (inr e)) = g_1 a) by apply (EqdepFacts.eq_sig_fst A).
-      contradict Hc.
-      unfold g_1, add_node_transport_1; case_if. }
-    rewrite Hin /add_node_transport_v_1.
-    case_if; destruct c; admit. (* Cas faux ! *)
-  - admit. (* Cas faux aussi ! *)
-Abort.
-
-Lemma add_node_transport_inj (c : comparison) (G : geos) (v0 v1 : G) (l : seq G)
+Lemma add_node_transport_inj (c : trilean) (G : geos) (v0 v1 : G) (l : seq G)
   (H : order G = v0 :: v1 :: l) :
   injective (add_node_transport c H).
 Proof.
@@ -1517,12 +1322,12 @@ Proof.
   by move => /eqP Heqbis; apply /eqP.
 Qed.
 
-Lemma add_node_transport_edges (c : comparison) (G : geos) (v0 v1 : G) (l : seq G)
+Lemma add_node_transport_edges (c : trilean) (G : geos) (v0 v1 : G) (l : seq G)
   (H : order G = v0 :: v1 :: l) :
   forall (v : G) (Hv : inl v \in
   (setT :\ inl (target (edge_of_concl v0)) :\ inl (target (edge_of_concl v1)) :
   {set add_node_graph_1 c (edge_of_concl v0) (edge_of_concl v1)})) (b : bool),
-  edges_at_subset b (Sub (inl v) Hv : add_node_graph_data c _ _)
+  edges_at_subset b (Sub (inl v) Hv : add_node_graph_data c _)
   = [set add_node_transport c H e | e in edges_at_subset b v].
 Proof.
   assert (vlabel v0 = concl_l /\ vlabel v1 = concl_l) as [Hv0  Hv1].
@@ -1547,7 +1352,7 @@ Proof.
       1: move => /andP[_ /andP[Hv _]].
       2: move => /andP[Hv _].
       all: contradict Hv; apply /negP; by rewrite negb_involutive. }
-  set w := Sub (inl v) Hv : add_node_graph_data c (add_node_hyp0 H) (add_node_hyp1 H).
+  set w := Sub (inl v) Hv : add_node_graph_data c (add_node_hyp H).
   set g := add_node_transport c H.
   set g_1 := add_node_transport_1 c e0 e1.
   set g_inj := add_node_transport_inj (c:=c) (H:=H).
@@ -1580,7 +1385,7 @@ Proof.
     by destruct b, c.
 Qed.
 
-Lemma add_node_transport_label (c : comparison) (G : geos) (v0 v1 : G) (l : seq G)
+Lemma add_node_transport_label (c : trilean) (G : geos) (v0 v1 : G) (l : seq G)
   (H : order G = v0 :: v1 :: l) : forall e,
   elabel (add_node_transport c H e) = elabel e.
 Proof.
@@ -1591,39 +1396,58 @@ Proof.
   unfold add_node_transport_1; case_if.
 Qed.
 
-Lemma add_node_p_deg (c : comparison) (G : geos) : proper_degree (add_node_graph_data_bis c G).
+Definition add_node_graph_data_bis : trilean -> geos -> graph_data :=
+  fun (c : trilean) (G : geos) =>
+  match order G as o return order G = o -> graph_data with
+  | v0 :: v1 :: _ => match c with
+                    | cut_t => if (elabel (edge_of_concl v0) == dual (elabel (edge_of_concl v1))) then
+                      fun Heq => add_node_graph_data c (add_node_hyp Heq)
+                      else fun _ => G
+                    | _ => fun Heq => add_node_graph_data c (add_node_hyp Heq)
+                    end
+  | _ => fun _ => G
+  end Logic.eq_refl. (* do nothing if inadequate *)
+
+(** Properties wished *)
+Lemma add_node_p_deg (c : trilean) (G : geos) : proper_degree (add_node_graph_data_bis c G).
 Proof.
   unfold add_node_graph_data_bis.
   generalize (erefl (order G));
   destruct (order G) as [ | v0 [ | v1 l]] at 2 3;
   intro H; try (apply p_deg).
+  revert c.
+  assert (forall c, proper_degree (add_node_graph_data c (add_node_hyp H))).
+  2:{ intros [ | | ]; trivial.
+      case_if.
+      apply p_deg. }
+  intro c.
   unfold proper_degree.
   intros b [[v | v] Hv]; cbn.
   - by rewrite (add_node_transport_edges H) -(p_deg b v)
-      -(card_imset (edges_at_subset b v) (add_node_transport_inj (c:=c) (H:=H))).
+      -(card_imset (edges_at_subset b v) (add_node_transport_inj (c := c) (H := H))).
   - set e0 := edge_of_concl v0; set e1 := edge_of_concl v1.
     set S := setT :\ inl (target e0) :\ inl (target e1) : {set add_node_graph_1 c e0 e1}.
     assert (None \in edge_set S /\ Some None \in edge_set S) as [Hn Hsn].
     { rewrite !in_set.
       split; repeat (apply /andP; split); trivial;
-      try (apply (add_node_hyp0 H) || apply (add_node_hyp1 H));
+      try apply (add_node_hyp H);
       by destruct c. }
-    set n := Sub None Hn : edge (add_node_graph_data c (add_node_hyp0 H) (add_node_hyp1 H));
-    set sn := Sub (Some None) Hsn : edge (add_node_graph_data c (add_node_hyp0 H) (add_node_hyp1 H)).
+    set n := Sub None Hn : edge (add_node_graph_data c (add_node_hyp H));
+    set sn := Sub (Some None) Hsn : edge (add_node_graph_data c (add_node_hyp H)).
     destruct c;
-    [set c := Eq | set c := Lt | set c := Gt].
+    [set c := tens_t | set c := parr_t | set c := cut_t].
     1,2: assert (Some (Some (inr None)) \in edge_set S /\ inr (inl tt) \in S /\ inr (inr tt) \in S)
           as [Hss [Htn Hcn]] by (rewrite !in_set; by repeat (split || apply /andP)).
-    1,2: set ss := Sub (Some (Some (inr None))) Hss : edge (add_node_graph_data c (add_node_hyp0 H) (add_node_hyp1 H));
-         set tn := Sub (inr (inl tt)) Htn : add_node_graph_data c (add_node_hyp0 H) (add_node_hyp1 H);
-         set cn := Sub (inr (inr tt)) Hcn : add_node_graph_data c (add_node_hyp0 H) (add_node_hyp1 H).
+    1,2: set ss := Sub (Some (Some (inr None))) Hss : edge (add_node_graph_data c (add_node_hyp H));
+         set tn := Sub (inr (inl tt)) Htn : add_node_graph_data c (add_node_hyp H);
+         set cn := Sub (inr (inr tt)) Hcn : add_node_graph_data c (add_node_hyp H).
     1,2: assert (edges_in_at_subset tn = [set n; sn] /\ edges_out_at_subset tn = [set ss] /\
                  edges_in_at_subset cn = [set ss] /\ edges_out_at_subset cn = set0)
           as [Htn_in [Htn_out [Hcn_in Hcn_out]]]
           by (repeat (split); apply /setP; intro e; rewrite !in_set;
             by destruct e as [[[[e | [[[] | []] | ]] | ] | ] ?]).
     3: assert (Htn : inr tt \in S) by (rewrite !in_set; apply /andP; by split).
-    3: set tn := (Sub (inr tt) Htn : add_node_graph_data c (add_node_hyp0 H) (add_node_hyp1 H)).
+    3: set tn := (Sub (inr tt) Htn : add_node_graph_data c (add_node_hyp H)).
     3: assert (edges_in_at_subset tn = [set n; sn] /\ edges_out_at_subset tn = set0)
         as [Htn_in Htn_out]
         by (split; apply /setP; intro e; rewrite !in_set; by destruct e as [[[[e | []] | ] | ] ?]).
@@ -1636,12 +1460,18 @@ Proof.
 Qed.
 Arguments add_node_p_deg : clear implicits.
 
-Lemma add_node_p_left (c : comparison) (G : geos) : proper_left (add_node_graph_data_bis c G).
+Lemma add_node_p_left (c : trilean) (G : geos) : proper_left (add_node_graph_data_bis c G).
 Proof.
   unfold add_node_graph_data_bis.
   generalize (erefl (order G));
   destruct (order G) as [ | v0 [ | v1 l]] at 2 3;
   intro H; try (apply p_left).
+  revert c.
+  assert (forall c, proper_left (add_node_graph_data c (add_node_hyp H))).
+  2:{ intros [ | | ]; trivial.
+      case_if.
+      apply p_left. }
+  intro c.
   assert (vlabel v0 = concl_l /\ vlabel v1 = concl_l) as [Hv0  Hv1].
   { destruct (p_order G) as [O _].
     split; [apply (O v0) | apply (O v1)];
@@ -1652,13 +1482,10 @@ Proof.
   intros [[v | v] Hv]; cbn;
   intro Hl; unfold add_node_left.
   - rewrite in_set; cbn.
-    rewrite !SubK !p_concl3 //.
-    assert (Hc : target (left v) = v).
-    { assert (Hcc : left v \in edges_in_at_subset v) by apply (p_left Hl).
-      apply /eqP; by rewrite in_set in Hcc. }
-    rewrite Hc.
-    case_if; apply /eqP; trivial;
-    destruct Hl as [Hl | Hl]; contradict Hl; by rewrite ?Hif ?Hif0 ?Hv0 ?Hv1.
+    rewrite !SubK !p_concl3 // p_left3 //.
+    case_if; apply /eqP; rewrite ?p_left3 //;
+    destruct Hl as [Hl | Hl];
+    contradict Hl; by rewrite ?Hif ?Hif0 ?Hv0 ?Hv1.
   - destruct c;
     [destruct v as [[] | []] | destruct v as [[] | []] | destruct v as []].
     all: try (destruct Hl as [Hl | Hl]; by contradict Hl).
@@ -1666,18 +1493,24 @@ Proof.
 Qed.
 Arguments add_node_p_left : clear implicits.
 
-Lemma add_node_p_order (c : comparison) (G : geos) : proper_order (add_node_graph_data_bis c G).
+Lemma add_node_p_order (c : trilean) (G : geos) : proper_order (add_node_graph_data_bis c G).
 Proof.
   unfold add_node_graph_data_bis.
   generalize (erefl (order G));
   destruct (order G) as [ | v0 [ | v1 l]] at 2 3;
   intro H; try (apply p_order).
+  revert c.
+  assert (forall c, proper_order (add_node_graph_data c (add_node_hyp H))).
+  2:{ intros [ | | ]; trivial.
+      case_if.
+      apply p_order. }
+  intro c.
   set e0 := edge_of_concl v0; set e1 := edge_of_concl v1.
   unfold proper_order.
   destruct (p_order G) as [Hv U].
   split; cbn.
   - intros [[v | v] Hin]; cbn;
-    rewrite /add_node_order map_id in_seq_sig SubK
+    rewrite /add_node_order in_seq_sig SubK
         -(proj2_sig (all_sigP (add_node_consistent_order c e0 e1))) /add_node_order_2.
     + apply (iff_stepl (A := v \in order G)). 2:{ by apply iff_sym. }
         assert (v != target e0 /\ v != target e1) as [Hv0 Hv1].
@@ -1691,214 +1524,50 @@ Proof.
           destruct c;
           rewrite ?in_cons /add_node_type_order/ add_node_order_1 mem_map //; cbn; trivial.
           all: by rewrite mem_filter Hv0 Hv1.
-    + destruct c.
-      3: destruct v as [].
-      1,2: destruct v as [[] | []].
-      all: cbn; split; trivial; intro Hl; contradict Hl; try by [].
-      all: rewrite ?in_cons /add_node_order_2 /add_node_type_order /add_node_order_1;
+    + destruct c;
+      [destruct v as [[] | []] | destruct v as [[] | []] | destruct v as []].
+      all: cbn; split; trivial; intro Hl; contradict Hl.
+      all: rewrite // ?in_cons /add_node_order_2 /add_node_type_order /add_node_order_1;
            cbn; apply /negP.
       all: apply inr_seq_inl_filter.
-  - rewrite /add_node_order map_id uniq_seq_sig
+  - rewrite /add_node_order uniq_seq_sig
       -(proj2_sig (all_sigP (add_node_consistent_order c e0 e1))) /add_node_order_2.
     destruct c;
     rewrite ?cons_uniq /add_node_type_order /add_node_order_1.
     1,2: apply /andP; split; [apply (inr_seq_inl_filter (order G) _ (inr tt)) | ].
     all: rewrite map_inj_uniq //; cbn; trivial; by apply filter_uniq.
 Qed.
+Arguments add_node_p_order : clear implicits.
 
-Definition add_node_geos (c : comparison) (G : geos) : geos := {|
+Definition add_node_geos (c : trilean) (G : geos) : geos := {|
   graph_data_of := add_node_graph_data_bis c G;
   p_deg := add_node_p_deg c G;
   p_left := add_node_p_left c G;
   p_order := add_node_p_order c G;
   |}.
 
-(******debut test part 1*************************************************************************************)
-(* Definition add_node_graph_data_bis' : comparison -> geos -> graph_data :=
-  fun (c : comparison) (G : geos) =>
-  match order G as o return order G = o -> graph_data with
-  | v0 :: v1 :: _ => if ((c != Gt) || (elabel (edge_of_concl v0) == elabel (edge_of_concl v1)^)) then
-                      fun Heq => add_node_graph_data c (add_node_hyp0 Heq) (add_node_hyp1 Heq)
-                      else fun _ => G
-  | _ => fun _ => G
-  end Logic.eq_refl. (* do nothing if inadequate *) TODO test is this way is easier *)
-Definition add_node_graph_data_bis' : comparison -> geos -> graph_data :=
-  fun (c : comparison) (G : geos) =>
-  match order G as o return order G = o -> graph_data with
-  | v0 :: v1 :: _ => match c with
-                     | Gt => if (elabel (edge_of_concl v0) == elabel (edge_of_concl v1)^) then
-                      fun Heq => add_node_graph_data c (add_node_hyp0 Heq) (add_node_hyp1 Heq)
-                      else fun _ => G
-                    | _ => fun Heq => add_node_graph_data c (add_node_hyp0 Heq) (add_node_hyp1 Heq)
-                    end
-  | _ => fun _ => G
-  end Logic.eq_refl. (* do nothing if inadequate *)
-Lemma add_node_p_deg' (c : comparison) (G : geos) : proper_degree (add_node_graph_data_bis' c G).
-Proof.
-  unfold add_node_graph_data_bis'.
-  generalize (erefl (order G));
-  destruct (order G) as [ | v0 [ | v1 l]] at 2 3;
-  intro H; try (apply p_deg).
-  revert c.
-  assert (Hm : forall c : comparison, proper_degree
-  (add_node_graph_data c (add_node_hyp0 H) (add_node_hyp1 H))).
-  2:{ intros [ | | ].
-      3: case_if; try (apply p_deg).
-      all: apply Hm. }
-  intro c.
-  destruct (add_node_hyp H) as [H0 H1].
-  unfold proper_degree.
-  intros b [[v | v] Hv]; cbn.
-  - by rewrite (add_node_transport_edges H) -(p_deg b v)
-      -(card_imset (edges_at_subset b v) (add_node_transport_inj (c:=c) (H:=H))).
-  - set e0 := edge_of_concl v0; set e1 := edge_of_concl v1.
-    set S := setT :\ inl (target e0) :\ inl (target e1) : {set add_node_graph_1 c e0 e1}.
-    assert (None \in edge_set S /\ Some None \in edge_set S) as [Hn Hsn].
-    { rewrite !in_set.
-      split; repeat (apply /andP; split); trivial;
-      try (apply H0 || apply H1);
-      by destruct c. }
-    set n := Sub None Hn : edge (add_node_graph_data c H0 H1);
-    set sn := Sub (Some None) Hsn : edge (add_node_graph_data c H0 H1).
-    destruct c;
-    [set c := Eq | set c := Lt | set c := Gt].
-    1,2: assert (Some (Some (inr None)) \in edge_set S /\ inr (inl tt) \in S /\ inr (inr tt) \in S)
-          as [Hss [Htn Hcn]] by (rewrite !in_set; by repeat (split || apply /andP)).
-    1,2: set ss := Sub (Some (Some (inr None))) Hss : edge (add_node_graph_data c H0 H1);
-         set tn := Sub (inr (inl tt)) Htn : add_node_graph_data c H0 H1;
-         set cn := Sub (inr (inr tt)) Hcn : add_node_graph_data c H0 H1.
-    1,2: assert (edges_in_at_subset tn = [set n; sn] /\ edges_out_at_subset tn = [set ss] /\
-                 edges_in_at_subset cn = [set ss] /\ edges_out_at_subset cn = set0)
-          as [Htn_in [Htn_out [Hcn_in Hcn_out]]]
-          by (repeat (split); apply /setP; intro e; rewrite !in_set;
-            by destruct e as [[[[e | [[[] | []] | ]] | ] | ] ?]).
-    3: assert (Htn : inr tt \in S) by (rewrite !in_set; apply /andP; by split).
-    3: set tn := (Sub (inr tt) Htn : add_node_graph_data c H0 H1).
-    3: assert (edges_in_at_subset tn = [set n; sn] /\ edges_out_at_subset tn = set0)
-        as [Htn_in Htn_out]
-        by (split; apply /setP; intro e; rewrite !in_set; by destruct e as [[[[e | []] | ] | ] ?]).
-    3: destruct v as [];
-      replace Hv with Htn by apply eq_irrelevance.
-    1,2: destruct v as [[] | []];
-      [replace Hv with Htn by apply eq_irrelevance | replace Hv with Hcn by apply eq_irrelevance].
-    all: destruct b; cbn.
-    all: by rewrite ?Htn_in ?Htn_out ?Hcn_in ?Hcn_out ?cards2 ?cards1 ?cards0.
-Qed.
-Arguments add_node_p_deg' : clear implicits.
-
-Lemma add_node_p_left' (c : comparison) (G : geos) : proper_left (add_node_graph_data_bis' c G).
-Proof.
-  unfold add_node_graph_data_bis'.
-  generalize (erefl (order G));
-  destruct (order G) as [ | v0 [ | v1 l]] at 2 3;
-  intro H; try (apply p_left).
-  revert c.
-  assert (Hm : forall c : comparison, proper_left
-  (add_node_graph_data c (add_node_hyp0 H) (add_node_hyp1 H))).
-  2:{ intros [ | | ].
-      3: case_if; try (apply p_left).
-      all: apply Hm. }
-  intro c.
-  assert (vlabel v0 = concl_l /\ vlabel v1 = concl_l) as [Hv0  Hv1].
-  { destruct (p_order G) as [O _].
-    split; [apply (O v0) | apply (O v1)];
-    rewrite H !in_cons eq_refl //.
-    apply /orP; by right. }
-  unfold proper_left.
-  destruct (add_node_hyp H).
-  intros [[v | v] Hv]; cbn;
-  intro Hl; unfold add_node_left.
-  - rewrite in_set; cbn.
-    rewrite !SubK !p_concl3 //.
-    assert (Hc : target (left v) = v).
-    { assert (Hcc : left v \in edges_in_at_subset v) by apply (p_left Hl).
-      apply /eqP; by rewrite in_set in Hcc. }
-    rewrite Hc.
-    case_if; apply /eqP; trivial;
-    destruct Hl as [Hl | Hl]; contradict Hl; by rewrite ?Hif ?Hif0 ?Hv0 ?Hv1.
-  - destruct c;
-    [destruct v as [[] | []] | destruct v as [[] | []] | destruct v as []].
-    all: try (destruct Hl as [Hl | Hl]; by contradict Hl).
-    all: by rewrite in_set !SubK.
-Qed.
-Arguments add_node_p_left' : clear implicits.
-
-Lemma add_node_p_order' (c : comparison) (G : geos) : proper_order (add_node_graph_data_bis' c G).
-Proof.
-  unfold add_node_graph_data_bis'.
-  generalize (erefl (order G));
-  destruct (order G) as [ | v0 [ | v1 l]] at 2 3;
-  intro H; try (apply p_order).
-  revert c.
-  assert (Hm : forall c : comparison, proper_order
-  (add_node_graph_data c (add_node_hyp0 H) (add_node_hyp1 H))).
-  2:{ intros [ | | ].
-      3: case_if; try (apply p_order).
-      all: apply Hm. }
-  intro c.
-  set e0 := edge_of_concl v0; set e1 := edge_of_concl v1.
-  unfold proper_order.
-  destruct (p_order G) as [Hv U].
-  split; cbn.
-  - intros [[v | v] Hin]; cbn;
-    rewrite /add_node_order map_id in_seq_sig SubK
-        -(proj2_sig (all_sigP (add_node_consistent_order c e0 e1))) /add_node_order_2.
-    + apply (iff_stepl (A := v \in order G)). 2:{ by apply iff_sym. }
-        assert (v != target e0 /\ v != target e1) as [Hv0 Hv1].
-        { split;
-          apply /negP; move => /eqP Hc;
-          contradict Hin; apply /negP;
-          rewrite Hc !in_set;
-          [apply /nandP; right | ];
-          apply /nandP; left;
-          by rewrite negb_involutive. }
-          destruct c;
-          rewrite ?in_cons /add_node_type_order/ add_node_order_1 mem_map //; cbn; trivial.
-          all: by rewrite mem_filter Hv0 Hv1.
-    + destruct c.
-      3: destruct v as [].
-      1,2: destruct v as [[] | []].
-      all: cbn; split; trivial; intro Hl; contradict Hl; try by [].
-      all: rewrite ?in_cons /add_node_order_2 /add_node_type_order /add_node_order_1;
-           cbn; apply /negP.
-      all: apply inr_seq_inl_filter.
-  - rewrite /add_node_order map_id uniq_seq_sig
-      -(proj2_sig (all_sigP (add_node_consistent_order c e0 e1))) /add_node_order_2.
-    destruct c;
-    rewrite ?cons_uniq /add_node_type_order /add_node_order_1.
-    1,2: apply /andP; split; [apply (inr_seq_inl_filter (order G) _ (inr tt)) | ].
-    all: rewrite map_inj_uniq //; cbn; trivial; by apply filter_uniq.
-Qed.
-Arguments add_node_p_order' : clear implicits.
-
-Definition add_node_geos' (c : comparison) (G : geos) : geos := {|
-  graph_data_of := add_node_graph_data_bis' c G;
-  p_deg := add_node_p_deg' c G;
-  p_left := add_node_p_left' c G;
-  p_order := add_node_p_order' c G;
-  |}.
-(******fin test part 1****************************************************************************************)
-
 
 
 (** ** Level 3: Proof Structure *)
 (** * The rule of a node gives conditions on the formulae of its arrows *)
 (* TODO factoriser proper_ax et cut aussi ?! *)
-Definition proper_ax (G : geos) :=
-  forall (v : G), vlabel v = ax_l -> exists el, exists er,
-  (el \in edges_out_at_subset v) && (er \in edges_out_at_subset v) &&
+Definition proper_ax_cut (G : geos) :=
+  forall (b : bool),
+  let rule := if b then cut_l else ax_l in
+  forall (v : G), vlabel v = rule -> exists el, exists er,
+  (el \in edges_at_subset b v) && (er \in edges_at_subset b v) &&
   (elabel el == dual (elabel er)).
 Lemma pre_proper_ax (G : geos) (v : G) (Hl : vlabel v = ax_l) :
   #|edges_out_at_subset v| = 2.
-Proof. by rewrite (p_deg_out v) Hl. Qed.
+Proof. by rewrite p_deg Hl. Qed.
 Definition proper_ax3 (G : geos) :=
   forall (v : G) (Hl : vlabel v = ax_l),
   true_on2 (is_dual_f (elabel (g := G))) (pre_proper_ax Hl).
-Lemma equiv_ax (G : geos) : proper_ax G -> proper_ax3 G.
+Lemma equiv_ax (G : geos) : proper_ax_cut G -> proper_ax3 G.
 Proof.
-  unfold proper_ax, proper_ax3.
+  unfold proper_ax_cut, proper_ax3.
   intros H v Hl.
-  elim: (H v Hl) => [el [er /andP[/andP[Hel Her] /eqP Heq]]].
+  elim: (H false v Hl) => [el [er /andP[/andP[Hel Her] /eqP Heq]]].
   assert (Ho : other (pre_proper_ax Hl) Hel = er).
   { apply p_other4; trivial.
     intro Hc.
@@ -1908,36 +1577,21 @@ Proof.
   by rewrite /is_dual_f /is_dual Ho Heq bidual.
 Qed.
 
-Definition proper_tens_parr (G : geos) :=
-  forall (b : bool),
-  let rule := if b then tens_l else parr_l in
-  let form := if b then tens else parr in
-  forall (v : G), vlabel v = rule ->
-  elabel (ccl v) = form (elabel (left v)) (elabel (right v)).
-(* OLD, TO REMOVE once sure
-Definition proper_tens (G : geos) :=
-  forall (v : G), vlabel v = tens_l ->
-  elabel (ccl v) = tens (elabel (left v)) (elabel (right v)).
-
-Definition proper_parr (G : geos) :=
-  forall (v : G), vlabel v = parr_l ->
-  elabel (ccl v) = parr (elabel (left v)) (elabel (right v)). *)
-
-Definition proper_cut (G : geos) :=
+(* Definition proper_cut (G : geos) :=
   forall (v : G), vlabel v = cut_l -> exists el, exists er,
   (el \in edges_in_at_subset v) && (er \in edges_in_at_subset v) &&
-  (elabel el == dual (elabel er)).
+  (elabel el == dual (elabel er)). *)
 Lemma pre_proper_cut (G : geos) (v : G) (Hl : vlabel v = cut_l) :
   #|edges_in_at_subset v| = 2.
-Proof. by rewrite (p_deg_in v) Hl. Qed.
+Proof. by rewrite p_deg Hl. Qed.
 Definition proper_cut3 (G : geos) :=
   forall (v : G) (Hl : vlabel v = cut_l),
   true_on2 (is_dual_f (elabel (g := G))) (pre_proper_cut Hl).
-Lemma equiv_cut (G : geos) : proper_cut G -> proper_cut3 G.
+Lemma equiv_cut (G : geos) : proper_ax_cut G -> proper_cut3 G.
 Proof.
-  unfold proper_cut, proper_cut3.
+  unfold proper_ax_cut, proper_cut3.
   intros H v Hl.
-  elim: (H v Hl) => [el [er /andP[/andP[Hel Her] /eqP Heq]]].
+  elim: (H true v Hl) => [el [er /andP[/andP[Hel Her] /eqP Heq]]].
   assert (Ho : other (pre_proper_cut Hl) Hel = er).
   { apply p_other4; trivial.
     intro Hc.
@@ -1948,41 +1602,40 @@ Proof.
   by rewrite /is_dual_f /is_dual Ho Heq bidual.
 Qed.
 
+Definition proper_tens_parr (G : geos) :=
+  forall (b : bool),
+  let rule := if b then parr_l else tens_l in
+  let form := if b then parr else tens in
+  forall (v : G), vlabel v = rule ->
+  elabel (ccl v) = form (elabel (left v)) (elabel (right v)).
+(* TODO modif bool dans proper_tens parr ?*)
+
 Set Primitive Projections.
 Record proof_structure : Type :=
   Proof_structure {
     geos_of :> geos;
-    p_ax : proper_ax geos_of;
+    p_ax_cut : proper_ax_cut geos_of;
     p_tens_parr : proper_tens_parr geos_of;
-    p_cut : proper_cut geos_of;
   }.
 Unset Primitive Projections.
-Definition p_tens (G : proof_structure) := @p_tens_parr G true.
-Definition p_parr (G : proof_structure) := @p_tens_parr G false.
+Definition p_ax (G : proof_structure) := @p_ax_cut G false.
+Definition p_cut (G : proof_structure) := @p_ax_cut G true.
+Definition p_tens (G : proof_structure) := @p_tens_parr G false.
+Definition p_parr (G : proof_structure) := @p_tens_parr G true.
 
 
 (** * The axiom graph is a proof_structure *)
-Lemma ax_p_ax (x : atom) : proper_ax (ax_geos x).
+Lemma ax_p_ax_cut (x : atom) : proper_ax_cut (ax_geos x).
 Proof.
-  unfold proper_ax.
-  intros v Hl.
+  unfold proper_ax_cut.
+  intros b v Hl.
+  destruct b;
   destruct_I3 v Hv;
   try (contradict Hl; by rewrite Hv).
   exists ord0, ord1.
-  by rewrite /edges_out_at_subset Hv 2!in_set !eq_refl.
+  by rewrite /edges_out_at_subset Hv !in_set !eq_refl.
 Qed.
-Lemma ax_p_ax3 (x : atom) : proper_ax3 (ax_geos x).
-Proof.
-  unfold proper_ax3.
-  intros v Hl.
-  destruct_I3 v Hv;
-  try (contradict Hl; by rewrite Hv).
-  assert (ord0 \in edges_out_at_subset v /\ ord1 \in edges_out_at_subset v) as [H0 H1]
-    by by rewrite /edges_out_at_subset Hv 2!in_set.
-  apply (simpl_sym (dual_sym_f (elabel (g:=ax_geos x))) (Ht := H0)).
-  by rewrite /is_dual_f /is_dual (p_other4 (y := ord1)).
-Qed.
-Arguments ax_p_ax : clear implicits.
+Arguments ax_p_ax_cut : clear implicits.
 
 Lemma ax_p_tens_parr (x : atom) : proper_tens_parr (ax_geos x).
 Proof.
@@ -1995,37 +1648,50 @@ Proof.
 Qed.
 Arguments ax_p_tens_parr : clear implicits.
 
-Lemma ax_p_cut (x : atom) : proper_cut (ax_geos x).
+Lemma ax_p_ax3 (x : atom) : proper_ax3 (ax_geos x).
 Proof.
-  unfold proper_cut.
+  unfold proper_ax3.
   intros v Hl.
   destruct_I3 v Hv;
-  contradict Hl;
-  by rewrite Hv.
+  try (contradict Hl; by rewrite Hv).
+  assert (ord0 \in edges_out_at_subset v /\ ord1 \in edges_out_at_subset v) as [H0 H1]
+    by by rewrite /edges_out_at_subset Hv !in_set.
+  apply (simpl_sym (dual_sym_f (elabel (g:=ax_geos x))) (Ht := H0)).
+  by rewrite /is_dual_f /is_dual (p_other4 (y := ord1)).
 Qed.
-Arguments ax_p_cut : clear implicits.
 
 Definition ax_ps (x : atom) : proof_structure := {|
   geos_of := ax_geos x;
-  p_ax := ax_p_ax x;
+  p_ax_cut := ax_p_ax_cut x;
   p_tens_parr := ax_p_tens_parr x;
-  p_cut := ax_p_cut x;
   |}.
 
 
 (** * A disjoint union of proof_structure is a proof_structure *)
-Lemma union_p_ax (G0 G1 : proof_structure) : proper_ax (union_geos G0 G1).
+Lemma union_p_ax_cut (G0 G1 : proof_structure) : proper_ax_cut (union_geos G0 G1).
 Proof.
-  unfold proper_ax.
-  intros [v | v] Hl; cbn; cbn in Hl.
-  all: destruct (p_ax Hl) as [el [er He]].
-  1: exists (inl el), (inl er); rewrite 2!union_edges_at_inl.
-  2: exists (inr el), (inr er); rewrite 2!union_edges_at_inr.
+  unfold proper_ax_cut.
+  intros b [v | v] Hl; cbn; cbn in Hl.
+  all: destruct (p_ax_cut Hl) as [el [er He]].
+  1: exists (inl el), (inl er); rewrite !union_edges_at_inl.
+  2: exists (inr el), (inr er); rewrite !union_edges_at_inr.
   all: rewrite !inj_imset //; by cbn.
 Qed.
+Arguments union_p_ax_cut : clear implicits.
+
+Lemma union_p_tens_parr (G0 G1 : proof_structure) : proper_tens_parr (union_geos G0 G1).
+Proof.
+  unfold proper_tens_parr.
+  intros [ | ] [v | v] Hl;
+  assert (vlabel v = tens_l \/ vlabel v = parr_l) by ((by left) || (by right));
+  rewrite union_right // union_ccl //;
+  by (apply p_tens || apply p_parr).
+Qed.
+Arguments union_p_tens_parr : clear implicits.
+
 Lemma union_p_ax3 (G0 G1 : proof_structure) : proper_ax3 (union_geos G0 G1).
 Proof.
-  assert (proper_ax3 G0 /\ proper_ax3 G1) as [H0 H1] by (split; apply equiv_ax, p_ax).
+  assert (proper_ax3 G0 /\ proper_ax3 G1) as [H0 H1] by (split; apply equiv_ax, p_ax_cut).
   (* TODO change the previous line when proper_ax chosen *)
   unfold proper_ax3.
   intros v Hl e He.
@@ -2051,30 +1717,10 @@ Proof.
         by apply /eqP).
   all: rewrite /is_dual_f /is_dual Hd Ho; by apply /eqP.
 Qed.
-Arguments union_p_ax : clear implicits.
 
-Lemma union_p_tens_parr (G0 G1 : proof_structure) : proper_tens_parr (union_geos G0 G1).
-Proof.
-  unfold proper_tens_parr.
-  intros [ | ] [v | v] Hl;
-  assert (vlabel v = tens_l \/ vlabel v = parr_l) by ((by left) || (by right));
-  rewrite union_right // union_ccl //;
-  by (apply p_tens || apply p_parr).
-Qed.
-Arguments union_p_tens_parr : clear implicits.
-
-Lemma union_p_cut (G0 G1 : proof_structure) : proper_cut (union_geos G0 G1).
-Proof.
-  unfold proper_cut.
-  intros [v | v] Hl; cbn; cbn in Hl.
-  all: destruct (p_cut Hl) as [el [er He]].
-  1: exists (inl el), (inl er); rewrite 2!union_edges_at_inl.
-  2: exists (inr el), (inr er); rewrite 2!union_edges_at_inr.
-  all: rewrite !inj_imset; by cbn.
-Qed.
 Lemma union_p_cut3 (G0 G1 : proof_structure) : proper_cut3 (union_geos G0 G1).
 Proof.
-  assert (proper_cut3 G0 /\ proper_cut3 G1) as [H0 H1] by (split; apply equiv_cut, p_cut).
+  assert (proper_cut3 G0 /\ proper_cut3 G1) as [H0 H1] by (split; apply equiv_cut, p_ax_cut).
   (* TODO change the previous line when proper_cut chosen *)
   unfold proper_cut3.
   intros v Hl e He.
@@ -2100,41 +1746,60 @@ Proof.
         by apply /eqP).
   all: rewrite /is_dual_f /is_dual Hd Ho; by apply /eqP.
 Qed.
-Arguments union_p_cut : clear implicits.
 
 Definition union_ps (G0 G1 : proof_structure) : proof_structure := {|
   geos_of := union_geos G0 G1;
-  p_ax := union_p_ax G0 G1;
+  p_ax_cut := union_p_ax_cut G0 G1;
   p_tens_parr := union_p_tens_parr G0 G1;
-  p_cut := union_p_cut G0 G1;
   |}.
 
 
 (** * Adding a node to a proof_structure yields a proof_structure *)
-Lemma add_node_p_ax (c : comparison) (G : proof_structure) : proper_ax (add_node_geos c G).
+Lemma add_node_p_ax_cut (c : trilean) (G : proof_structure) : proper_ax_cut (add_node_geos c G).
 Proof.
   remember (order G) as l eqn:H; symmetry in H.
-  unfold add_node_geos, add_node_graph_data_bis, proper_ax; cbn.
-  assert (Hdone : forall (v : match l return (order G = l -> graph_data) with
+  unfold add_node_geos, add_node_graph_data_bis, proper_ax_cut; cbn.
+  assert (Hdone : forall (b : bool) (v : match l return (order G = l -> graph_data) with
     | [::] => fun=> G
-    | v' :: l' => match l' return (order G = v' :: l' -> graph_data) with
+    | v0 :: l0 => match l0 return (order G = v0 :: l0 -> graph_data) with
       | [::] => fun=> G
-      | v'' :: l'' => fun Heq : order G = [:: v', v'' & l''] =>
-        add_node_graph_data c (add_node_hyp0 Heq) (add_node_hyp1 Heq)
-    end end H), vlabel v = ax ->
+      | v1 :: l1 => match c with
+              | cut_t => if (elabel (edge_of_concl v0)) == (elabel (edge_of_concl v1)^)
+                      then fun Heq : order G = [:: v0, v1 & l1] =>
+                      add_node_graph_data c (add_node_hyp Heq)
+                      else fun=> G
+              | _ => fun Heq : order G = [:: v0, v1 & l1] =>
+                     add_node_graph_data c (add_node_hyp Heq)
+    end end end H), vlabel v = (if b then cut else ax) ->
   exists (el er : edge (match l return (order G = l -> graph_data) with
     | [::] => fun=> G
-    | v' :: l' => match l' return (order G = v' :: l' -> graph_data) with
+    | v0 :: l0 => match l0 return (order G = v0 :: l0 -> graph_data) with
       | [::] => fun=> G
-      | v'' :: l'' => fun Heq : order G = [:: v', v'' & l''] =>
-        add_node_graph_data c (add_node_hyp0 Heq) (add_node_hyp1 Heq)
-    end end H)), (el \in edges_out_at_subset v) && (er \in edges_out_at_subset v) &&
+      | v1 :: l1 => match c with
+              | cut_t => if (elabel (edge_of_concl v0)) == (elabel (edge_of_concl v1)^)
+                      then fun Heq : order G = [:: v0, v1 & l1] =>
+                      add_node_graph_data c (add_node_hyp Heq)
+                      else fun=> G
+              | _ => fun Heq : order G = [:: v0, v1 & l1] =>
+                     add_node_graph_data c (add_node_hyp Heq)
+    end end end H)), (el \in edges_at_subset b v) && (er \in edges_at_subset b v) &&
   (elabel el == dual (elabel er))).
   2:{ by rewrite <-!H in Hdone. }
   destruct l as [ | v0 [ | v1 l]];
-  try (apply p_ax).
-  intros [[v | v] Hv] Hl; cbn in Hl; cbn.
-  - elim (p_ax Hl) => el [er /andP[/andP[Hel Her] /eqP Helr]].
+  try (apply p_ax_cut).
+  assert (Hdone : c <> cut_t \/ elabel (edge_of_concl v0) = dual (elabel (edge_of_concl v1)) ->
+    forall b (v : add_node_graph_data c (add_node_hyp H)),
+    vlabel v = (if b then cut else ax) -> exists el er : edge (add_node_graph_data c (add_node_hyp H)),
+    (el \in edges_at_subset b v) && (er \in edges_at_subset b v) && (elabel el == elabel er^)).
+  2:{ case_if.
+      - replace (match c with | tens_t | _ => fun Heq : order G = [:: v0, v1 & l] =>
+        add_node_graph_data c (add_node_hyp Heq) end H) with
+        (add_node_graph_data c (add_node_hyp H)) by by destruct c.
+        apply Hdone; by right.
+      - destruct c;
+        [apply Hdone; by left | apply Hdone; by left | apply p_ax_cut]. }
+  intros Hor b [[v | v] Hv] Hl; cbn in Hl; cbn.
+  - elim (p_ax_cut Hl) => el [er /andP[/andP[Hel Her] /eqP Helr]].
     exists (add_node_transport c H el), (add_node_transport c H er).
     rewrite !(add_node_transport_edges H) !inj_imset ?Hel ?Her;
     [ | apply add_node_transport_inj | apply add_node_transport_inj]; cbn.
@@ -2144,42 +1809,67 @@ Proof.
     all: contradict Helr;
       rewrite ?Hif ?Hif0 ?Hif1 ?Hif2;
       apply nesym, no_selfdual.
-  - contradict Hl; by destruct c, v.
+  - destruct b, c, v;
+    try (by contradict Hl).
+    set e0 := edge_of_concl v0; set e1 := edge_of_concl v1.
+    set S := setT :\ inl (target e0) :\ inl (target e1) : {set add_node_graph_1 cut_t e0 e1}.
+    assert (None \in edge_set S /\ Some None \in edge_set S) as [Hn Hsn].
+    { rewrite !in_set.
+      split; repeat (apply /andP; split); trivial;
+      apply (add_node_hyp H). }
+    set n := Sub None Hn : edge (add_node_graph_data cut_t (add_node_hyp H));
+    set sn := Sub (Some None) Hsn : edge (add_node_graph_data cut_t (add_node_hyp H)).
+    exists n, sn.
+    assert (elabel e1 == dual (elabel e0))
+      by (destruct Hor as [Hc | Heq]; by rewrite // Heq bidual).
+    rewrite !in_set; cbn; by rewrite !SubK.
 Qed.
-Arguments add_node_p_ax : clear implicits.
+Arguments add_node_p_ax_cut : clear implicits.
 
-Lemma add_node_p_tens_parr (c : comparison) (G : proof_structure) : proper_tens_parr (add_node_geos c G).
+Lemma add_node_p_tens_parr (c : trilean) (G : proof_structure) : proper_tens_parr (add_node_geos c G).
 Proof.
   remember (order G) as l eqn:H; symmetry in H.
   unfold add_node_geos, add_node_graph_data_bis.
-  intros b r f v Hv; rewrite ccl_eq ?right_eq; 
-  [ | destruct b; [by left | by right] | destruct b; [by left | by right]];
+  intros b r f v Hv; rewrite ccl_eq ?right_eq;
+  [ | destruct b; [by right | by left] | destruct b; [by right | by left]];
   revert v Hv; cbn.
   assert (Hdone : forall (v : match l return (order G = l -> graph_data) with
     | [::] => fun=> G
-    | v' :: l' => match l' return (order G = v' :: l' -> graph_data) with
+    | v0 :: l0 => match l0 return (order G = v0 :: l0 -> graph_data) with
       | [::] => fun=> G
-      | v'' :: l'' => fun Heq : order G = [:: v', v'' & l''] =>
-        add_node_graph_data c (add_node_hyp0 Heq) (add_node_hyp1 Heq)
-    end end H), vlabel v = r -> elabel (ccl' v) = f (elabel (left v)) (elabel (right' v))).
+      | v1 :: l1 => match c with
+              | cut_t => if (elabel (edge_of_concl v0)) == (elabel (edge_of_concl v1)^)
+                      then fun Heq : order G = [:: v0, v1 & l1] =>
+                      add_node_graph_data c (add_node_hyp Heq)
+                      else fun=> G
+              | _ => fun Heq : order G = [:: v0, v1 & l1] =>
+                     add_node_graph_data c (add_node_hyp Heq)
+    end end end H), vlabel v = r -> elabel (ccl' v) = f (elabel (left v)) (elabel (right' v))).
   2:{ by rewrite <-!H in Hdone. }
   destruct l as [ | v0 [ | v1 l]];
   intros v Hv;
-  assert (Hor : vlabel v = tens_l \/ vlabel v = parr_l) by (destruct b; [by left | by right]);
+  assert (Hor : vlabel v = tens_l \/ vlabel v = parr_l) by (destruct b; [by right | by left]);
   try (rewrite -ccl_eq // -right_eq //; by apply p_tens_parr).
-  destruct v as [[v | v] Hin].
+  revert c v Hv Hor.
+  assert (Hdone : forall c (v : add_node_graph_data c (add_node_hyp H)),
+    vlabel v = r -> vlabel v = ⊗ \/ vlabel v = ⅋ ->
+    elabel (ccl' v) = f (elabel (left v)) (elabel (right' v))).
+  2:{ intros [ | | ];
+      [specialize (Hdone tens_t) | specialize (Hdone parr_t) | specialize (Hdone cut_t)]; trivial.
+      case_if; rewrite -?Hif //.
+      intros; rewrite -ccl_eq // -right_eq //; by apply p_tens_parr. }
+  intros c [[v | v] Hin] Hv Hor.
   - cbn in Hv; cbn in Hor.
-    set w := Sub (inl v) Hin : add_node_graph_data c (add_node_hyp0 H) (add_node_hyp1 H).
-    assert (Hc := p_left Hor); revert Hc; rewrite in_set; move => /eqP Hc.
+    set w := Sub (inl v) Hin : add_node_graph_data c (add_node_hyp H).
     assert (Hneq := Hin); rewrite !in_set in Hneq; cbn in Hneq;
     revert Hneq; move => /andP[/eqP Hneq0 /andP[/eqP Hneq1 _]].
     replace (elabel (left w)) with (elabel (left v)).
     2:{ cbn; rewrite !SubK /add_node_left_1.
         case_if.
-        - by rewrite -Hif Hc in Hneq1.
-        - by rewrite -Hif0 Hc in Hneq0. }
+        - by rewrite -Hif p_left3 in Hneq1.
+        - by rewrite -Hif0 p_left3 in Hneq0. }
     assert (ccl' w \in edges_out_at_subset w /\ right' w \in edges_in_at_subset w :\ left w)
-      as [Hccl Hright].
+      as [Hccl Hright]. (* TODO voir si lemma general *)
     { unfold ccl', right'.
       split;
       [destruct [pick x in edges_out_at_subset w] as [e | ] eqn:He |
@@ -2212,20 +1902,19 @@ Proof.
       { elim (p_order G).
         rewrite H cons_uniq in_cons negb_or.
         by move => _ /andP[/andP[/eqP ? _] _]. }
-      assert (target (left v) <> target (edge_of_concl v0) /\
+       assert (target (left v) <> target (edge_of_concl v0) /\
         target (left v) <> target (edge_of_concl v1)) as [Hc0 Hc1].
-      { rewrite Hc.
-        split; intro Hf;
-        contradict Hv; by rewrite ?Hv0 ?Hv1. }
+        by rewrite p_left3 //.
       case_if.
       + rewrite !p_concl3 // in Hif0.
         by rewrite Hif0 in Hneqv.
-      + contradict Hc1.
-        by rewrite Hif.
+      + contradict Hv.
+        rewrite -(p_left3 Hor) Hif p_concl3 // Hv1.
+        by destruct b.
       + by []. }
     by apply p_tens_parr.
   - destruct c;
-    [set c := Eq | set c := Lt | set c := Gt];
+    [set c := tens_t | set c := parr_t | set c := cut_t];
     [destruct v as [[] | []] | destruct v as [[] | []] | destruct v as []];
     destruct b;
     try (by contradict Hv).
@@ -2237,10 +1926,10 @@ Proof.
       repeat ((apply /andP; split) || split); trivial;
       try (apply (add_node_hyp H));
       by destruct c).
-    all: set n := Sub None Hn : edge (add_node_graph_data c (add_node_hyp0 H) (add_node_hyp1 H));
-      set sn := Sub (Some None) Hsn : edge (add_node_graph_data c (add_node_hyp0 H) (add_node_hyp1 H));
-      set ss := Sub (Some (Some (inr None))) Hss : edge (add_node_graph_data c (add_node_hyp0 H) (add_node_hyp1 H));
-      set tn := Sub (inr (inl tt)) Hin : add_node_graph_data c (add_node_hyp0 H) (add_node_hyp1 H).
+    all: set n := Sub None Hn : edge (add_node_graph_data c (add_node_hyp H));
+      set sn := Sub (Some None) Hsn : edge (add_node_graph_data c (add_node_hyp H));
+      set ss := Sub (Some (Some (inr None))) Hss : edge (add_node_graph_data c (add_node_hyp H));
+      set tn := Sub (inr (inl tt)) Hin : add_node_graph_data c (add_node_hyp H).
     all: assert (edges_in_at_subset tn = [set n; sn] /\ edges_out_at_subset tn = [set ss])
           as [Htn_in Htn_out]
           by (split; apply /setP; intro e; rewrite !in_set; by destruct e as [[[[e | [[[] | []] | ]] | ] | ] ?]).
@@ -2263,222 +1952,18 @@ Proof.
 Qed.
 Arguments add_node_p_tens_parr : clear implicits.
 
-(******debut test part 2**************************************************************************************)
-Lemma add_node_p_ax' (c : comparison) (G : proof_structure) : proper_ax (add_node_geos' c G).
-Proof.
-Admitted.
-Arguments add_node_p_ax' : clear implicits.
-
-Lemma add_node_p_tens_parr' (c : comparison) (G : proof_structure) : proper_tens_parr (add_node_geos' c G).
-Proof.
-Admitted.
-Arguments add_node_p_tens_parr' : clear implicits.
-
-Lemma add_node_p_cut' (c : comparison) (G : proof_structure) : proper_cut (add_node_geos' c G).
-Proof.
-  remember (order G) as l eqn:H; symmetry in H.
-  unfold add_node_geos', add_node_graph_data_bis', proper_cut; cbn.
-  assert (Hdone : 
-  forall (v : match l return (order G = l -> graph_data) with
-    | [::] => fun=> G
-    | v0 :: l0 => match l0 return (order G = v0 :: l0 -> graph_data) with
-      | [::] => fun=> G
-      | v1 :: l1 => match c with
-                   | Gt =>
-                       if
-                        eqb_form (elabel (edge_of_concl v0))
-                          (elabel (edge_of_concl v1)^)
-                       then
-                        fun Heq : order G = [:: v0, v1 & l1] =>
-                        add_node_graph_data c (add_node_hyp0 Heq)
-                          (add_node_hyp1 Heq)
-                       else fun=> G
-                   | _ =>
-                       fun Heq : order G = [:: v0, v1 & l1] =>
-                       add_node_graph_data c (add_node_hyp0 Heq)
-                         (add_node_hyp1 Heq)
-                   end
-    end end H), vlabel v = cut ->
-  exists (el er : edge (match l return (order G = l -> graph_data) with
-    | [::] => fun=> G
-    | v0 :: l0 => match l0 return (order G = v0 :: l0 -> graph_data) with
-      | [::] => fun=> G
-      | v1 :: l1 => match c with
-                   | Gt =>
-                       if
-                        eqb_form (elabel (edge_of_concl v0))
-                          (elabel (edge_of_concl v1)^)
-                       then
-                        fun Heq : order G = [:: v0, v1 & l1] =>
-                        add_node_graph_data c (add_node_hyp0 Heq)
-                          (add_node_hyp1 Heq)
-                       else fun=> G
-                   | _ =>
-                       fun Heq : order G = [:: v0, v1 & l1] =>
-                       add_node_graph_data c (add_node_hyp0 Heq)
-                         (add_node_hyp1 Heq)
-                   end
-    end end H)), (el \in edges_in_at_subset v) && (er \in edges_in_at_subset v) &&
-  (elabel el == dual (elabel er))).
-  2:{ by rewrite <-!H in Hdone. }
-  destruct l as [ | v0 [ | v1 l]];
-  try (apply p_cut).
-  case_if.
-{ rename Hif into Hdual.
-  replace (match c with | Eq | _ => fun Heq : order G = [:: v0, v1 & l] =>
-    add_node_graph_data c (add_node_hyp0 Heq) (add_node_hyp1 Heq) end H) with
-    (add_node_graph_data c (add_node_hyp0 H) (add_node_hyp1 H)) by by destruct c.
-  intros [[v | v] Hv] Hl; cbn in Hl; cbn.
-  - elim (p_cut Hl) => el [er /andP[/andP[Hel Her] /eqP Helr]].
-    exists (add_node_transport c H el), (add_node_transport c H er).
-    rewrite !(add_node_transport_edges H) !inj_imset ?Hel ?Her;
-    [ | apply add_node_transport_inj | apply add_node_transport_inj]; cbn.
-    rewrite /add_node_transport !SubK /add_node_transport_1.
-    case_if; apply /eqP.
-    all: try by rewrite -?Hif -?Hif0 -?Hif1 -?Hif2.
-    all: contradict Helr;
-      rewrite ?Hif ?Hif0 ?Hif1 ?Hif2;
-      apply nesym, no_selfdual.
-  - destruct c;
-    try (contradict Hl; by destruct v).
-    destruct v.
-    set e0 := edge_of_concl v0; set e1 := edge_of_concl v1.
-    set S := setT :\ inl (target e0) :\ inl (target e1) : {set add_node_graph_1 Gt e0 e1}.
-    set H0 := add_node_hyp0 H; set H1 := add_node_hyp1 H.
-    assert (None \in edge_set S /\ Some None \in edge_set S) as [Hn Hsn].
-    { rewrite !in_set.
-      split; repeat (apply /andP; split); trivial;
-      apply (add_node_hyp H). }
-    set n := Sub None Hn : edge (add_node_graph_data Gt H0 H1);
-    set sn := Sub (Some None) Hsn : edge (add_node_graph_data Gt H0 H1).
-    exists n, sn.
-    assert (elabel e1 == dual (elabel e0)) by by rewrite Hdual bidual.
-    rewrite !in_set; cbn; by rewrite !SubK.
-}
-{ clear Hif.
-  revert c.
-  assert (Hm : forall c, c <> Gt -> forall v : add_node_graph_data c (add_node_hyp0 H) (add_node_hyp1 H),
-  vlabel v = cut -> exists el er : edge (add_node_graph_data c (add_node_hyp0 H) (add_node_hyp1 H)),
-  (el \in edges_in_at_subset v) && (er \in edges_in_at_subset v) && eqb_form (elabel el) (elabel er^)).
-  2:{ intros [ | | ]; try apply p_cut; by apply Hm. }
-  intros c Hc.
-  intros [[v | v] Hv] Hl; cbn in Hl; cbn.
-  - elim (p_cut Hl) => el [er /andP[/andP[Hel Her] /eqP Helr]].
-    exists (add_node_transport c H el), (add_node_transport c H er).
-    rewrite !(add_node_transport_edges H) !inj_imset ?Hel ?Her;
-    [ | apply add_node_transport_inj | apply add_node_transport_inj]; cbn.
-    rewrite /add_node_transport !SubK /add_node_transport_1.
-    case_if; apply /eqP.
-    all: try by rewrite -?Hif -?Hif0 -?Hif1 -?Hif2.
-    all: contradict Helr;
-      rewrite ?Hif ?Hif0 ?Hif1 ?Hif2;
-      apply nesym, no_selfdual.
-  - destruct c;
-    contradict Hl; by destruct v.
-}
-Qed.
-Arguments add_node_p_cut' : clear implicits.
-
-Definition add_node_ps' (c : comparison) (G : proof_structure) :
-  proof_structure := {|
-  geos_of := add_node_geos' c G;
-  p_ax := add_node_p_ax' c G;
-  p_tens_parr := add_node_p_tens_parr' c G;
-  p_cut := add_node_p_cut' c G;
-  |}.
-(* TODO ça marche sans la condition :) -> à finir *)
-(****fin test part 2******************************************************************************************)
-
-(* Necessary condition on formulas when adding a node cut *)
-Definition add_node_cond (c : comparison) (G : proof_structure) : bool.
-Proof.
-  destruct (order G) as [ | v0 [ | v1 l]] eqn:H.
-  - apply true.
-  - apply true.
-  - destruct c.
-    + apply true.
-    + apply true.
-    + apply (elabel (edge_of_concl v0) == dual (elabel (edge_of_concl v1))).
-Defined.
-(* TOTEST lorsqu'on ajoute un cut, ne le faire que si les formules correspondent *)
-
-Lemma add_node_p_cut (c : comparison) (G : proof_structure) (Hcut : add_node_cond c G) :
-  proper_cut (add_node_geos c G).
-Proof.
-  revert Hcut.
-  remember (order G) as l eqn:H; symmetry in H.
-  unfold add_node_geos, add_node_graph_data_bis, proper_cut, add_node_cond; cbn.
-  assert (Hdone : match l return (order G = l -> bool) with
-    | [::] => xpredT
-    | v0 :: l' => match l' return (order G = v0 :: l' -> bool) with
-      | [::] => xpredT
-      | v1 :: l1 => fun=> match c with
-        | Gt => elabel (edge_of_concl v0) == dual (elabel (edge_of_concl v1))
-        | _ => true
-    end end end H ->
-  forall (v : match l return (order G = l -> graph_data) with
-    | [::] => fun=> G
-    | v' :: l' => match l' return (order G = v' :: l' -> graph_data) with
-      | [::] => fun=> G
-      | v'' :: l'' => fun Heq : order G = [:: v', v'' & l''] =>
-        add_node_graph_data c (add_node_hyp0 Heq) (add_node_hyp1 Heq)
-    end end H), vlabel v = cut ->
-  exists (el er : edge (match l return (order G = l -> graph_data) with
-    | [::] => fun=> G
-    | v' :: l' => match l' return (order G = v' :: l' -> graph_data) with
-      | [::] => fun=> G
-      | v'' :: l'' => fun Heq : order G = [:: v', v'' & l''] =>
-        add_node_graph_data c (add_node_hyp0 Heq) (add_node_hyp1 Heq)
-    end end H)), (el \in edges_in_at_subset v) && (er \in edges_in_at_subset v) &&
-  (elabel el == dual (elabel er))).
-  2:{ by rewrite <-!H in Hdone. }
-  destruct l as [ | v0 [ | v1 l]];
-  move => Hcut;
-  try (apply p_cut).
-  intros [[v | v] Hv] Hl; cbn in Hl; cbn.
-  - elim (p_cut Hl) => el [er /andP[/andP[Hel Her] /eqP Helr]].
-    exists (add_node_transport c H el), (add_node_transport c H er).
-    rewrite !(add_node_transport_edges H) !inj_imset ?Hel ?Her;
-    [ | apply add_node_transport_inj | apply add_node_transport_inj]; cbn.
-    rewrite /add_node_transport !SubK /add_node_transport_1.
-    case_if; apply /eqP.
-    all: try by rewrite -?Hif -?Hif0 -?Hif1 -?Hif2.
-    all: contradict Helr;
-      rewrite ?Hif ?Hif0 ?Hif1 ?Hif2;
-      apply nesym, no_selfdual.
-  - destruct c;
-    try (contradict Hl; by destruct v).
-    destruct v.
-    set e0 := edge_of_concl v0; set e1 := edge_of_concl v1.
-    set S := setT :\ inl (target e0) :\ inl (target e1) : {set add_node_graph_1 Gt e0 e1}.
-    set H0 := add_node_hyp0 H; set H1 := add_node_hyp1 H.
-    assert (None \in edge_set S /\ Some None \in edge_set S) as [Hn Hsn].
-    { rewrite !in_set.
-      split; repeat (apply /andP; split); trivial;
-      apply (add_node_hyp H). }
-    set n := Sub None Hn : edge (add_node_graph_data Gt H0 H1);
-    set sn := Sub (Some None) Hsn : edge (add_node_graph_data Gt H0 H1).
-    exists n, sn.
-    assert (elabel e1 == dual (elabel e0)) by by rewrite (eqP Hcut) bidual.
-    rewrite !in_set; cbn; by rewrite !SubK.
-Qed.
-Arguments add_node_p_cut : clear implicits.
-
-Definition add_node_ps (c : comparison) (G : proof_structure) (H : add_node_cond c G) :
-  proof_structure := {|
+Definition add_node_ps (c : trilean) (G : proof_structure) : proof_structure := {|
   geos_of := add_node_geos c G;
-  p_ax := add_node_p_ax c G;
+  p_ax_cut := add_node_p_ax_cut c G;
   p_tens_parr := add_node_p_tens_parr c G;
-  p_cut := add_node_p_cut c G H;
   |}.
-Arguments add_node_ps : clear implicits.
 
 
 
 (** ** Proof Structure of a Proof Sequent *)
 (* TOTHINK mettre les ax, union, add_node ici ? *)
 
-(** * Permuting the conclusions of a geos or a proof_structure *)
+(** * Permuting the conclusions of a geos *)
 (** Function taking two lists l1 l2 permutations of one another, and returning a polymorphic permutation sending l1 to l2 *)
 Fixpoint perm_of {A : Type} {l1 l2 : seq A} (sigma : Permutation_Type l1 l2) {struct sigma} :
   forall {B : Type}, seq B -> seq B :=
@@ -2499,11 +1984,8 @@ Lemma perm_of_consistent {A : Type} {l1 l2 : seq A} (sigma : Permutation_Type l1
   perm_of sigma l1 = l2.
 Proof.
   unfold perm_of.
-  induction sigma as [ | x l l' sigma H | x y l | l l' l'' sigma H sigma' H'].
-  - by [].
-  - by rewrite H.
-  - by [].
-  - by rewrite H H'.
+  induction sigma as [ | x l l' sigma H | x y l | l l' l'' sigma H sigma' H'];
+  by rewrite ?H ?H' //.
 Qed.
 
 Lemma perm_of_map : forall {A B S : Type} (l : seq A) (f : A -> B) (l1 l2 : seq S) (sigma : Permutation_Type l1 l2),
@@ -2514,13 +1996,13 @@ Proof.
   induction sigma as [ | x l l' sigma H | x y l | l l' l'' sigma H sigma' H']; cbn;
   intros A B l0 f.
   - by [].
-  - destruct l0; cbn; by rewrite ?H.
+  - destruct l0; cbn; by rewrite // H.
   - by destruct l0 as [ | a [ | b l0]].
   - by rewrite H H'.
 Qed.
 
 Lemma perm_of_in {A : Type} {l1 l2 : seq A} (sigma : Permutation_Type l1 l2) :
-  forall  {B : finType} (l : seq B) (b : B), (b \in perm_of sigma l) = (b \in l).
+  forall {B : finType} (l : seq B) (b : B), (b \in perm_of sigma l) = (b \in l).
 Proof.
   induction sigma as [ | x l l' sigma H | x y l | l l' l'' sigma H sigma' H']; cbn;
   intros B l0 b.
@@ -2606,8 +2088,8 @@ Proof.
     trivial.
   all: try (contradict H; by rewrite H').
   all: replace H' with H by apply eq_irrelevance.
-  all: try set to := tens_to_tensparr H.
-  all: try set to := parr_to_tensparr H.
+  all: try set to := tens_to_tensparr H;
+       try set to := parr_to_tensparr H.
   all: try replace (perm_p_left sigma v to) with (p_left to) by apply eq_irrelevance.
   all: try by replace (@unique_right (perm_geos G sigma) v to) with (@unique_right G v to)
     by apply eq_irrelevance.
@@ -2617,10 +2099,10 @@ Proof.
     by apply eq_irrelevance.
 Qed.
 
-Lemma perm_p_ax (G : proof_structure) (l l' : list formula) (sigma : Permutation_Type l l') :
-  proper_ax (perm_geos G sigma).
-Proof. apply p_ax. Qed.
-Arguments perm_p_ax {G} {l l'} (sigma).
+Lemma perm_p_ax_cut (G : proof_structure) (l l' : list formula) (sigma : Permutation_Type l l') :
+  proper_ax_cut (perm_geos G sigma).
+Proof. apply p_ax_cut. Qed.
+Arguments perm_p_ax_cut {G} {l l'} (sigma).
 
 Lemma perm_p_tens_parr (G : proof_structure) (l l' : list formula) (sigma : Permutation_Type l l') :
   proper_tens_parr (perm_geos G sigma).
@@ -2633,38 +2115,31 @@ Proof.
 Qed.
 Arguments perm_p_tens_parr {G} {l l'} (sigma).
 
-Lemma perm_p_cut (G : proof_structure) (l l' : list formula) (sigma : Permutation_Type l l') :
-  proper_cut (perm_geos G sigma).
-Proof. apply p_cut. Qed.
-Arguments perm_p_cut {G} {l l'} (sigma).
-
 Definition perm_ps (G : proof_structure) (l l' : list formula) (sigma : Permutation_Type l l') :
   proof_structure := {|
   geos_of := perm_geos G sigma;
-  p_ax := perm_p_ax sigma;
+  p_ax_cut := perm_p_ax_cut sigma;
   p_tens_parr := perm_p_tens_parr sigma;
-  p_cut := perm_p_cut sigma;
   |}.
 
-Lemma ax_sequent (X : atom) : sequent (ax_ps X) = covar X :: var X :: nil.
+Lemma ax_sequent (x : atom) : sequent (ax_geos x) = covar x :: var x :: nil.
 Proof.
   unfold sequent.
-  replace ([seq elabel (edge_of_concl i) | i <- order (ax_ps X)]) with
-    ([:: elabel (edge_of_concl (ord1 : ax_ps X)); elabel (edge_of_concl (ord2 : ax_ps X))]) by by [].
-  assert (edge_of_concl (ord1 : ax_ps X) = ord0 /\ edge_of_concl (ord2 : ax_ps X) = ord1) as [H1 H2].
-  { assert (Hin : (ord0 : edge (ax_ps X)) \in edges_in_at_subset (ord1 : ax_ps X)
-      /\ (ord1 : edge (ax_ps X)) \in edges_in_at_subset (ord2 : ax_ps X))
+  replace ([seq elabel (edge_of_concl i) | i <- order (ax_geos x)]) with
+    ([:: elabel (edge_of_concl (ord1 : ax_geos x)); elabel (edge_of_concl (ord2 : ax_geos x))]) by by [].
+  assert (edge_of_concl (ord1 : ax_geos x) = ord0 /\ edge_of_concl (ord2 : ax_geos x) = ord1) as [H1 H2].
+  { assert (Hin : (ord0 : edge (ax_geos x)) \in edges_in_at_subset (ord1 : ax_geos x)
+      /\ (ord1 : edge (ax_geos x)) \in edges_in_at_subset (ord2 : ax_geos x))
       by (split; by rewrite in_set).
     revert Hin; rewrite !p_concl2 // !in_set; by move => [/eqP ? /eqP ?]. }
   by rewrite H1 H2.
 Qed.
 
-Lemma perm_sequent (G : proof_structure) (l l' : list formula) (sigma : Permutation_Type l l') (Heq : (sequent G) = l) :
-  sequent (perm_ps G sigma) = l'.
+Lemma perm_sequent (G : proof_structure) (l l' : list formula) (sigma : Permutation_Type l l')
+  (Heq : (sequent G) = l) : sequent (perm_geos G sigma) = l'.
 Proof.
-  revert sigma; rewrite <-!Heq; intro sigma.
-  unfold perm_ps; cbn.
-  rewrite -perm_of_map; cbn.
+  revert sigma; rewrite <-!Heq; intro sigma; cbn.
+  rewrite -perm_of_map.
   destruct (perm_simpl G sigma) as [_ [_ He]].
   replace (@map G formula (fun i : G => @elabel _ _ G (@edge_of_concl (@perm_geos G (sequent G) l' sigma) i))
         (order G)) with (@map G formula (fun i : G => @elabel _ _ G (@edge_of_concl G i)) (order G))
@@ -2672,15 +2147,15 @@ Proof.
   apply perm_of_consistent.
 Qed.
 
-Lemma union_sequent (G0 G1 : proof_structure) : sequent (union_ps G0 G1) =
+Lemma union_sequent (G0 G1 : geos) : sequent (union_geos G0 G1) =
   match sequent G0, sequent G1 with
   | f0 :: s0, f1 :: s1 => f0 :: f1 :: s1 ++ s0
   | _, [::] => sequent G0
   | [::], _ => sequent G1
   end.
 Proof.
-  assert ((forall v, edge_of_concl (inr v : union_ps G0 G1) = inr (edge_of_concl v))
-        /\ forall v, edge_of_concl (inl v : union_ps G0 G1) = inl (edge_of_concl v))
+  assert ((forall v, edge_of_concl (inr v : union_geos G0 G1) = inr (edge_of_concl v))
+        /\ forall v, edge_of_concl (inl v : union_geos G0 G1) = inl (edge_of_concl v))
         as [Hr Hl].
   { split; intro v;
     destruct (vlabel v) eqn:Hv.
@@ -2695,141 +2170,287 @@ Proof.
       intro H';
       try (contradict H'; by rewrite Hv);
       by [].
-    1: assert (H : inr (edge_of_concl v) \in edges_in_at_subset (inr v : union_ps G0 G1))
+    1: assert (H : inr (edge_of_concl v) \in edges_in_at_subset (inr v : union_geos G0 G1))
       by (rewrite union_edges_at_inr inj_imset; [ | apply inr_inj]; by apply p_concl).
-    2: assert (H : inl (edge_of_concl v) \in edges_in_at_subset (inl v : union_ps G0 G1))
+    2: assert (H : inl (edge_of_concl v) \in edges_in_at_subset (inl v : union_geos G0 G1))
       by (rewrite union_edges_at_inl inj_imset; [ | apply inl_inj]; by apply p_concl).
     all: rewrite p_concl2 // in_set in H.
-    all: symmetry; by apply /eqP. }
+    all: symmetry; by apply /eqP. } (* TODO lemme *)
   cbn; unfold union_order, sequent.
   destruct (order G0) as [ | v0 o0];
   destruct (order G1) as [ | v1 o1];
   trivial; cbn.
   all: rewrite ?Hr ?Hl.
   all: apply /eqP; rewrite !eqseq_cons !eq_refl; apply /andP; split; trivial; apply /eqP.
-  all: try (induction o1 as [ | ? ? H1]; trivial; cbn).
-  all: try (induction o0 as [ | ? ? H0]; trivial; cbn).
-  all: by rewrite ?H1 ?H0 ?Hr ?Hl.
+all: rewrite ?map_cat -!map_comp /comp ?map_id.
+all: try replace ([seq match edge_of_concl (inl x : union_geos G0 G1) with
+      | inl e => elabel e | inr e => elabel e end | x <- o0])
+      with ([seq elabel (edge_of_concl i) | i <- o0])
+      by (apply eq_map; intros ?; by rewrite ?Hr ?Hl);
+     try replace ([seq match edge_of_concl (inr x : union_geos G0 G1) with
+      | inl e => elabel e | inr e => elabel e end | x <- o1])
+      with ([seq elabel (edge_of_concl i) | i <- o1])
+      by (apply eq_map; intros ?; by rewrite ?Hr ?Hl);
+     trivial.
 Qed.
 
-Lemma add_node_sequent (c : comparison) (G : proof_structure) (H : add_node_cond c G) :
+Lemma add_node_sequent (c : trilean) (G : geos) :
   let new := match order G with
     | v0 :: v1 :: _ => match c with
-      | Eq => [:: tens (elabel (edge_of_concl v0)) (elabel (edge_of_concl v1))]
-      | Lt => [:: parr (elabel (edge_of_concl v0)) (elabel (edge_of_concl v1))]
-      | Gt => nil (*TODO ajouter condition dual *)
+      | tens_t => [:: tens (elabel (edge_of_concl v0)) (elabel (edge_of_concl v1))]
+      | parr_t => [:: parr (elabel (edge_of_concl v0)) (elabel (edge_of_concl v1))]
+      | cut_t => nil
       end
     | _ => nil
     end in
   let old := match order G with
-    | v0 :: v1 :: _ => behead (behead (sequent G))
+    | v0 :: v1 :: _ => match c with 
+      | cut_t => if (elabel (edge_of_concl v0)) == (elabel (edge_of_concl v1)^)
+              then behead (behead (sequent G))
+              else sequent G
+      | _ => behead (behead (sequent G))
+      end
     | _ => sequent G
     end in
-  sequent (add_node_ps c G H) = new ++ old.
+  sequent (add_node_geos c G) = new ++ old.
 Proof.
+  remember (order G) as l eqn:H; symmetry in H.
+  unfold add_node_geos, add_node_graph_data_bis. cbn.
+  assert([seq elabel (edge_of_concl' i)
+   | i <- order
+            (match order G as o return (order G = o -> graph_data) with
+             | [::] => fun=> G
+             | v0 :: l =>
+                 match
+                   l as l0 return (order G = v0 :: l0 -> graph_data)
+                 with
+                 | [::] => fun=> G
+                 | v1 :: l0 =>
+                     match c with
+                     | cut_t =>
+                         if
+                          eqb_form (elabel (edge_of_concl' v0))
+                            (elabel (edge_of_concl' v1)^)
+                         then
+                          fun Heq : order G = [:: v0, v1 & l0] =>
+                          add_node_graph_data c 
+                            (add_node_hyp Heq)
+                         else fun=> G
+                     | _ =>
+                         fun Heq : order G = [:: v0, v1 & l0] =>
+                         add_node_graph_data c 
+                           (add_node_hyp Heq)
+                     end
+                 end
+             end (erefl (order G)))] =
+match order G with
+| [::] => [::]
+| [:: v0] => [::]
+| [:: v0, v1 & _] =>
+    match c with
+    | tens_t => [:: elabel (edge_of_concl' v0) ⊗ elabel (edge_of_concl' v1)]
+    | parr_t => [:: elabel (edge_of_concl' v0) ⅋ elabel (edge_of_concl' v1)]
+    | cut_t => [::]
+    end
+end ++
+match order G with
+| [::] => sequent G
+| [:: v0] => sequent G
+| [:: v0, v1 & _] =>
+    match c with
+    | cut_t =>
+        if
+         eqb_form (elabel (edge_of_concl' v0))
+           (elabel (edge_of_concl' v1)^)
+        then behead (behead (sequent G))
+        else sequent G
+    | _ => behead (behead (sequent G))
+    end
+end
+).
+2:{ admit. (*rewrite <-!edge_of_concl_eq.*) }
+assert (Hdone : [seq elabel (edge_of_concl' i)
+   | i <- order
+            (match l as o return (order G = o -> graph_data) with
+             | [::] => fun=> G
+             | v0 :: l0 =>
+                 match l0 as l1 return (order G = v0 :: l1 -> graph_data) with
+                 | [::] => fun=> G
+                 | v1 :: l1 =>
+                     match c with
+                     | cut_t =>
+                         if
+                          eqb_form (elabel (edge_of_concl' v0))
+                            (elabel (edge_of_concl' v1)^)
+                         then
+                          fun Heq : order G = [:: v0, v1 & l1] =>
+                          add_node_graph_data c (add_node_hyp Heq)
+                         else fun=> G
+                     | _ =>
+                         fun Heq : order G = [:: v0, v1 & l1] =>
+                         add_node_graph_data c (add_node_hyp Heq)
+                     end
+                 end
+             end H)] =
+match l with
+| [::] => [::]
+| [:: v0] => [::]
+| [:: v0, v1 & _] =>
+    match c with
+    | tens_t => [:: elabel (edge_of_concl' v0) ⊗ elabel (edge_of_concl' v1)]
+    | parr_t => [:: elabel (edge_of_concl' v0) ⅋ elabel (edge_of_concl' v1)]
+    | cut_t => [::]
+    end
+end ++
+match l with
+| [::] => sequent G
+| [:: v0] => sequent G
+| [:: v0, v1 & _] =>
+    match c with
+    | cut_t =>
+        if eqb_form (elabel (edge_of_concl' v0)) (elabel (edge_of_concl' v1)^)
+        then behead (behead (sequent G))
+        else sequent G
+    | _ => behead (behead (sequent G))
+    end
+end).
+2:{ by rewrite <-!H in Hdone. }
+  destruct l as [ | v0 [ | v1 l0]].
+  - by rewrite /sequent !H.
+  - rewrite /sequent !H; cbn.
+    rewrite -edge_of_concl_eq //.
+    destruct (p_order G) as [O _].
+    apply O.
+    rewrite H in_cons.
+    apply /orP; by left.
+  - destruct c.
+    + rewrite /sequent H; cbn.
+      rewrite /add_node_order.
+assert (Hm :=(proj2_sig (all_sigP (add_node_consistent_order tens_t (edge_of_concl v0) (edge_of_concl v1))))).
+unfold add_node_graph_1 in Hm. cbn in Hm. cbn.
+(* assert (forall (i : (add_node_graph_data tens_t (add_node_hyp H))), (@sval) (option (option (edge G + option (void + void))))
+         (fun x : option (option (edge G + option (void + void))) =>
+          x
+            \in edge_set
+                  (setT :\ inl (target (edge_of_concl v0))
+                   :\ inl (target (edge_of_concl v1)) : {set add_node_graph_1 tens_t (edge_of_concl v0) (edge_of_concl v1)})) 
+         (edge_of_concl' i) = (edge_of_concl' (sval i))). *)
+(* TODO passer par un intermediaire avec map ( map) *)
+(* rewrite -Hm. *)
+(* rewrite SubK. *)
+(* rewrite /add_node_type_order /add_node_order_1 in Hm. *)
+(*     rewrite /add_node_order map_id in_seq_sig SubK
+        -(proj2_sig (all_sigP (add_node_consistent_order c e0 e1))) /add_node_order_2.
+      rewrite eqseq_cons. *)
+(* replace ([seq elabel (edge_of_concl' i) | i <- order G])
+with ([seq elabel (edge_of_concl i) | i <- order G]) . done.
+rewrite H.
+apply eq_map; intros ?; rewrite -edge_of_concl_eq //. *)
 Admitted.
 
-Lemma add_node_cond_tens : forall (G : proof_structure), add_node_cond Eq G.
-Proof.
-  unfold add_node_cond.
-  intro G.
-  generalize (erefl (order G));
-  by destruct (order G) as [ | v0 [ | v1 l]] at 2 3.
-Qed.
-
-Lemma add_node_cond_parr : forall (G : proof_structure), add_node_cond Lt G.
-Proof.
-  unfold add_node_cond.
-  intro G.
-  generalize (erefl (order G));
-  by destruct (order G) as [ | v0 [ | v1 l]] at 2 3.
-Qed.
-Lemma add_node_cond_cut : forall (G : proof_structure), add_node_cond Gt G.
-Admitted. (*FAUX*)
-(** * Traduction of a sequant proof into a proof structure *)
+(** * Traduction of a sequent proof into a proof structure *)
 Fixpoint ps {l : list formula} (pi : ll l) : proof_structure := match pi with
-| ax_r x => ax_ps x
-| ex_r _ _ pi0 sigma => perm_ps (ps pi0) sigma
-| tens_r _ _ _ _ pi0 pi1 => add_node_ps Eq (union_ps (ps pi0) (ps pi1)) (add_node_cond_tens (union_ps (ps pi0) (ps pi1)))
-| parr_r _ _ _ pi0 => add_node_ps Lt (ps pi0) (add_node_cond_parr (ps pi0))
-| cut_r _ _ _ pi0 pi1 => add_node_ps Gt (union_ps (ps pi0) (ps pi1)) (add_node_cond_cut (union_ps (ps pi0) (ps pi1)))
-end. (* TODO virer lemma faux + prouver ça avec sequent OU faire plus general que la condition *)
-
-(*debut test part 3*****************)
-Fixpoint ps' {l : list formula} (pi : ll l) : proof_structure := match pi with
-| ax_r x => ax_ps x
-| ex_r _ _ pi0 sigma => perm_ps (ps' pi0) sigma
-| tens_r _ _ _ _ pi0 pi1 => add_node_ps' Eq (union_ps (ps' pi0) (ps' pi1))
-| parr_r _ _ _ pi0 => add_node_ps' Lt (ps' pi0)
-| cut_r _ _ _ pi0 pi1 => add_node_ps' Gt (union_ps (ps' pi0) (ps' pi1))
-end.
-
-Lemma ps_consistent' {l : list formula} (pi : ll l) : sequent (ps' pi) = l.
-Proof.
-  induction pi as [x | l l' pi0 H0 sigma | A B l0 l1 pi0 H0 pi1 H1 | A B l0 pi0 H0 | A l0 l1 pi0 H0 pi1 H1].
-  - apply ax_sequent.
-  - apply (perm_sequent sigma H0).
-  - admit.
-  - admit. (* idem tens *)
-  - admit.
-Admitted.
-(*fin test part 3*************)
+  | ax_r x => ax_ps x
+  | ex_r _ _ pi0 sigma => perm_ps (ps pi0) sigma
+  | tens_r _ _ _ _ pi0 pi1 => add_node_ps tens_t (union_ps (ps pi0) (ps pi1))
+  | parr_r _ _ _ pi0 => add_node_ps parr_t (ps pi0)
+  | cut_r _ _ _ pi0 pi1 => add_node_ps cut_t (union_ps (ps pi0) (ps pi1))
+  end.
 
 Lemma ps_consistent {l : list formula} (pi : ll l) : sequent (ps pi) = l.
 Proof.
   induction pi as [x | l l' pi0 H0 sigma | A B l0 l1 pi0 H0 pi1 H1 | A B l0 pi0 H0 | A l0 l1 pi0 H0 pi1 H1].
   - apply ax_sequent.
-  - apply (perm_sequent sigma H0).
+  - by apply perm_sequent.
   - rewrite add_node_sequent union_sequent H0 H1.
-    cbn. unfold union_order.
-(*     destruct (order ((fix ps (l : seq formula) (pi : ⊢ l) {struct pi} : proof_structure :=
+    cbn; unfold union_order.
+    destruct (order ((fix ps (l : seq formula) (pi : ⊢ l) {struct pi} : proof_structure :=
           match pi with
           | ax_r x => ax_ps x
-          | @ex_r l0 l3 pi0 sigma => perm_ps (ps l0 pi0) sigma
-          | @tens_r A0 B0 l0 l3 pi0 pi3 =>
-              add_node_ps Eq (union_ps (ps (A0 :: l0) pi0) (ps (B0 :: l3) pi3))
-                (add_node_cond_tens
-                   (union_ps (ps (A0 :: l0) pi0) (ps (B0 :: l3) pi3)))
-          | @parr_r A0 B0 l0 pi0 =>
-              add_node_ps Lt (ps [:: A0, B0 & l0] pi0)
-                (add_node_cond_parr (ps [:: A0, B0 & l0] pi0))
-          | @cut_r A0 l0 l3 pi0 pi3 =>
-              add_node_ps Gt (union_ps (ps (A0 :: l0) pi0) (ps (A0^ :: l3) pi3))
-                (add_node_cond_cut
-                   (union_ps (ps (A0 :: l0) pi0) (ps (A0^ :: l3) pi3)))
-          end) (A :: l1) pi1)) eqn:H1.
-    1:{ contradict IHpi1; by rewrite /sequent H1. }
-    destruct (order
-      ((fix ps (l0 : seq formula) (pi : ⊢ l0) {struct pi} : proof_structure :=
+          | @ex_r l2 l3 pi2 sigma => perm_ps (ps l2 pi2) sigma
+          | @tens_r A0 B0 l2 l3 pi2 pi3 => add_node_ps tens_t (union_ps (ps (A0 :: l2) pi2) (ps (B0 :: l3) pi3))
+          | @parr_r A0 B0 l2 pi2 => add_node_ps parr_t (ps [:: A0, B0 & l2] pi2)
+          | @cut_r A0 l2 l3 pi2 pi3 => add_node_ps cut_t (union_ps (ps (A0 :: l2) pi2) (ps (A0^ :: l3) pi3))
+          end) (A :: l0) pi0)) as [ | v0 o0] eqn:Ho0.
+    1:{ contradict H0; by rewrite /sequent Ho0. }
+    destruct (order ((fix ps (l2 : seq formula) (pi : ⊢ l2) {struct pi} : proof_structure :=
           match pi with
           | ax_r x => ax_ps x
-          | @ex_r l3 l4 pi0 sigma => perm_ps (ps l3 pi0) sigma
-          | @tens_r A0 B0 l3 l4 pi0 pi3 =>
-              add_node_ps Eq (union_ps (ps (A0 :: l3) pi0) (ps (B0 :: l4) pi3))
-                (add_node_cond_tens
-                   (union_ps (ps (A0 :: l3) pi0) (ps (B0 :: l4) pi3)))
-          | @parr_r A0 B0 l3 pi0 =>
-              add_node_ps Lt (ps [:: A0, B0 & l3] pi0)
-                (add_node_cond_parr (ps [:: A0, B0 & l3] pi0))
-          | @cut_r A0 l3 l4 pi0 pi3 =>
-              add_node_ps Gt (union_ps (ps (A0 :: l3) pi0) (ps (A0^ :: l4) pi3))
-                (add_node_cond_cut
-                   (union_ps (ps (A0 :: l3) pi0) (ps (A0^ :: l4) pi3)))
-          end) (B :: l2) pi2)) eqn:H2.
-    1:{ contradict IHpi2; by rewrite /sequent H2. }
-    assert (vlabel s = concl_l /\ vlabel s0 = concl_l) as [Hc1 Hc2] by admit. (* same as v0 v1 *)
-    rewrite !union_edge_of_concl //. (*TODO merge proof union_right & ccl & concl *)
-    assert (elabel (edge_of_concl s) = A /\ elabel (edge_of_concl s0) = B) as [He1 He2].
+          | @ex_r l3 l4 pi2 sigma => perm_ps (ps l3 pi2) sigma
+          | @tens_r A0 B0 l3 l4 pi2 pi3 => add_node_ps tens_t (union_ps (ps (A0 :: l3) pi2) (ps (B0 :: l4) pi3))
+          | @parr_r A0 B0 l3 pi2 => add_node_ps parr_t (ps [:: A0, B0 & l3] pi2)
+          | @cut_r A0 l3 l4 pi2 pi3 => add_node_ps cut_t (union_ps (ps (A0 :: l3) pi2) (ps (A0^ :: l4) pi3))
+          end) (B :: l1) pi1)) as [ | v1 o1] eqn:Ho1.
+    1:{ contradict H1; by rewrite /sequent Ho1. }
+    assert (vlabel v0 = concl_l /\ vlabel v1 = concl_l) as [Hv0  Hv1].
+      { split;
+        [destruct (p_order (ps pi0)) as [O _] |destruct (p_order (ps pi1)) as [O _]];
+        apply O;
+        rewrite ?Ho0 ?Ho1 !in_cons eq_refl //. }
+    rewrite !union_edge_of_concl //.
+    assert (elabel (edge_of_concl v0) = A /\ elabel (edge_of_concl v1) = B) as [He1 He2].
     { split;
-      [assert (Hv := IHpi1) | assert (Hv := IHpi2)].
-      all: rewrite /sequent ?H1 ?H2 in Hv.
+      [assert (Hv := H0) | assert (Hv := H1)].
+      all: rewrite /sequent ?Ho0 ?Ho1 in Hv.
       all: revert Hv; move => /eqP Hv; cbn in Hv.
       all: revert Hv; by move => /andP [/eqP Hv _]. }
-    by rewrite He1 He2. *)
-    admit.
-  - admit. (* idem tens *)
-  - admit.
-Admitted.
+    by rewrite He1 He2.
+  - rewrite add_node_sequent H0.
+    destruct (order ((fix ps (l : seq formula) (pi : ⊢ l) {struct pi} : proof_structure :=
+          match pi with
+          | ax_r x => ax_ps x
+          | @ex_r l2 l3 pi2 sigma => perm_ps (ps l2 pi2) sigma
+          | @tens_r A0 B0 l2 l3 pi2 pi3 => add_node_ps tens_t (union_ps (ps (A0 :: l2) pi2) (ps (B0 :: l3) pi3))
+          | @parr_r A0 B0 l2 pi2 => add_node_ps parr_t (ps [:: A0, B0 & l2] pi2)
+          | @cut_r A0 l2 l3 pi2 pi3 => add_node_ps cut_t (union_ps (ps (A0 :: l2) pi2) (ps (A0^ :: l3) pi3))
+          end) [:: A, B & l0] pi0)) as [ | v0 [ | v1 o]] eqn:Ho.
+    1,2: contradict H0; by rewrite /sequent Ho.
+      assert (vlabel v0 = concl_l /\ vlabel v1 = concl_l) as [Hv0  Hv1].
+      { destruct (p_order (ps pi0)) as [O _].
+        split; apply O;
+        rewrite Ho !in_cons eq_refl //.
+        apply /orP; by right. }
+    assert (elabel (edge_of_concl v0) = A /\ elabel (edge_of_concl v1) = B) as [He1 He2].
+    { rewrite /sequent Ho in H0.
+      revert H0; move => /eqP H0; cbn in H0.
+      revert H0; by move => /andP [/eqP H0 /andP[/eqP H1 _]]. }
+    by rewrite He1 He2.
+  - rewrite add_node_sequent union_sequent H0 H1.
+    cbn; unfold union_order.
+    destruct (order ((fix ps (l : seq formula) (pi : ⊢ l) {struct pi} : proof_structure :=
+          match pi with
+          | ax_r x => ax_ps x
+          | @ex_r l2 l3 pi2 sigma => perm_ps (ps l2 pi2) sigma
+          | @tens_r A0 B0 l2 l3 pi2 pi3 => add_node_ps tens_t (union_ps (ps (A0 :: l2) pi2) (ps (B0 :: l3) pi3))
+          | @parr_r A0 B0 l2 pi2 => add_node_ps parr_t (ps [:: A0, B0 & l2] pi2)
+          | @cut_r A0 l2 l3 pi2 pi3 => add_node_ps cut_t (union_ps (ps (A0 :: l2) pi2) (ps (A0^ :: l3) pi3))
+          end) (A :: l0) pi0)) as [ | v0 o0] eqn:Ho0.
+    1:{ contradict H0; by rewrite /sequent Ho0. }
+    destruct (order ((fix ps (l2 : seq formula) (pi : ⊢ l2) {struct pi} :  proof_structure :=
+          match pi with
+          | ax_r x => ax_ps x
+          | @ex_r l3 l4 pi2 sigma => perm_ps (ps l3 pi2) sigma
+          | @tens_r A0 B0 l3 l4 pi2 pi3 => add_node_ps tens_t (union_ps (ps (A0 :: l3) pi2) (ps (B0 :: l4) pi3))
+          | @parr_r A0 B0 l3 pi2 => add_node_ps parr_t (ps [:: A0, B0 & l3] pi2)
+          | @cut_r A0 l3 l4 pi2 pi3 => add_node_ps cut_t (union_ps (ps (A0 :: l3) pi2) (ps (A0^ :: l4) pi3))
+          end) (dual A :: l1) pi1)) as [ | v1 o1] eqn:Ho1.
+    1:{ contradict H1; by rewrite /sequent Ho1. }
+    assert (vlabel v0 = concl_l /\ vlabel v1 = concl_l) as [Hv0  Hv1].
+      { split;
+        [destruct (p_order (ps pi0)) as [O _]
+        |destruct (p_order (ps pi1)) as [O _]];
+        apply O;
+        rewrite ?Ho0 ?Ho1 !in_cons eq_refl //. }
+    rewrite !union_edge_of_concl //.
+    assert (elabel (edge_of_concl v0) = A /\ elabel (edge_of_concl v1) = dual A) as [He1 He2].
+    { split;
+      [assert (Hv := H0) | assert (Hv := H1)].
+      all: rewrite /sequent ?Ho0 ?Ho1 in Hv.
+      all: revert Hv; move => /eqP Hv; cbn in Hv.
+      all: revert Hv; by move => /andP [/eqP Hv _]. }
+    rewrite He1 He2 bidual.
+    case_if.
+Qed.
 
 
 
@@ -2859,6 +2480,7 @@ Lemma sound l (pi : ll l) : is_correct ps (pi).
 *)
 
 (** ** Cut Elimination *)
+(* possible avant la sequentialisation et le critere de correction *)
 (*
 Inductive red : 
 | ax->cut: merge the 2 nodes, then merge the final node with the node above,
@@ -2880,217 +2502,5 @@ Inductive red :
 (* function to turn a ps into a sequential proof *)
 
 (* TODO check if every lemma proved is useful / interesting *)
-
-
-(**************************************************************************************************)
-(** ** PREVIOUS CONTENT of the file mll.v *)
-
-(** * Cut Elimination *)
-
-Ltac destruct_eqrefl H :=
-list_simpl in H;
-match goal with
-| H : ?x = ?x |- _ => assert (H = eq_refl) as ->
-                        by apply (Eqdep_dec.UIP_dec (@eq_dt_dec (list_dectype formulas_dectype)));
-                      cbn
-end.
-
-(** Symmetric induction principle *)
-Lemma sym_induction_ll (P : forall [A B l1 l2 l3 l4], ll (l1 ++ A :: l2) -> ll (l3 ++ B :: l4)
-                          -> Type) :
-  (forall A B l1 l2 l3 l4 (pi1 : ll (l1 ++ A :: l2)) (pi2 : ll (l3 ++ B :: l4)),
-     P pi2 pi1 -> P pi1 pi2) ->
-  (forall X B l3 l4 (pi2 : ll (l3 ++ B :: l4)),
-     P (ax_r X : ll (nil ++ covar X :: var X :: nil)) pi2) ->
-  (forall X B l3 l4 (pi2 : ll (l3 ++ B :: l4)),
-     P (ax_r X : ll ((covar X :: nil) ++ var X :: nil)) pi2) ->
-  (forall A B l1 l2 l3 l4 l' (pi1 : ll l') (pi2 : ll (l3 ++ B :: l4))
-     (HP : Permutation_Type l' (l1 ++ A :: l2)),
-     P (rew (rew (surjective_pairing (proj1_sig (Permutation_Type_vs_elt_inv _ _ _ HP)))
-              in proj2_sig (Permutation_Type_vs_elt_inv _ _ _ HP)) in pi1) pi2 ->
-     P (ex_r pi1 HP) pi2) ->
-  (forall A B C D l0 l1 l2 l3 l4 (pi0 : ll (C :: l0))
-     (pi1 : ll (D :: l1 ++ A :: l2)) (pi2 : ll (l3 ++ B :: l4)),
-     P (pi1 : ll ((D :: l1) ++ A :: l2)) pi2 ->
-     P (rew <- (app_assoc (tens C D :: l1) (A :: l2) _) in tens_r pi0 pi1) pi2) ->
-  (forall A B C D l0 l1 l2 l3 l4 (pi0 : ll (D :: l0))
-     (pi1 : ll (C :: l1 ++ A :: l2)) (pi2 : ll (l3 ++ B :: l4)),
-     P (pi1 : ll ((C :: l1) ++ A :: l2)) pi2 ->
-     P (rew (app_assoc (tens C D :: l0) _ (A :: l2)) in tens_r pi1 pi0 ) pi2) ->
-  (forall A B C D l1 l2 l3 l4 (pi1 : ll (C :: D :: l1 ++ A :: l2)) (pi2 : ll (l3 ++ B :: l4)),
-     P (pi1 : ll ((C :: D :: l1) ++ A :: l2)) pi2 ->
-     P (parr_r pi1 : ll ((parr C D :: l1) ++ A :: l2)) pi2) ->
-  (forall C D C' D' l2' l2'' (pi1' : ll (C :: l2')) (pi1'' : ll (D :: l2'')),
-     (forall l3 l4 (pi2 : ll (l3 ++ C' :: l4)), P (pi1' : ll (nil ++ _)) pi2) ->
-     (forall l3 l4 (pi2 : ll (l3 ++ D' :: l4)), P (pi1'' : ll (nil ++ _)) pi2) ->
-     forall l4' l4'' (pi2' : ll (C' :: l4')) (pi2'' : ll (D' :: l4'')),
-       P (tens_r pi1' pi1'' : ll (nil ++ _)) (tens_r pi2' pi2'' : ll (nil ++ _))) ->
-  (forall C D C' D' l2 (pi1 : ll (C :: D :: l2)),
-     (forall l3 l4 (pi2 : ll (l3 ++ C' :: l4)), P (pi1 : ll (nil ++ _)) pi2) ->
-      forall l4 (pi2 : ll (C' :: D' :: l4)),
-       P (parr_r pi1 : ll (nil ++ _)) (parr_r pi2 : ll (nil ++ _))) ->
-  (forall C D C' D' l1' l1'' (pi1' : ll (C :: l1')) (pi1'' : ll (D :: l1'')),
-     (forall l3 l4 (pi2 : ll (l3 ++ C' :: l4)), P (pi1' : ll (nil ++ _)) pi2) ->
-     (forall l3 l4 (pi2 : ll (l3 ++ D' :: l4)), P (pi1'' : ll (nil ++ _)) pi2) ->
-     forall l4 (pi2 : ll (D' :: C' :: l4)),
-       P (tens_r pi1' pi1'' : ll (nil ++ _)) (parr_r pi2 : ll (nil ++ _))) ->
-  forall A B l1 l2 l3 l4 (pi1 : ll (l1 ++ A :: l2)) (pi2 : ll (l3 ++ B :: l4)), P pi1 pi2.
-Proof.
-intros Hsym Hax1 Hax2 Hex Htens1 Htens2 Hparr Htt Hpp Htp.
-enough (forall c s A B s1 s2 (pi1 : ll s1) (pi2 : ll s2),
-          s = psize pi1 + psize pi2 -> fsize A <= c -> fsize B <= c ->
-          forall l1 l2 l3 l4 (Heq1 : s1 = l1 ++ A :: l2) (Heq2 : s2 = l3 ++ B :: l4),
-          P A B l1 l2 l3 l4 (rew Heq1 in pi1) (rew Heq2 in pi2)) as IH
-  by (now intros A B l1 l2 l3 l4 pi1 pi2;
-          refine (IH (max (fsize A) (fsize B)) _ _ _ _ _ pi1 pi2 _ _ _ _ _ _ _ eq_refl eq_refl);
-          try lia).
-induction c as [c IHf0] using lt_wf_rect.
-assert (forall A B, fsize A < c -> fsize B < c ->
-          forall l1 l2 l3 l4 pi1 pi2, P A B l1 l2 l3 l4 pi1 pi2) as IHf
-  by (now intros A B HA HB l1 l2 l3 l4 pi1 pi2;
-          refine (IHf0 (max (fsize A) (fsize B)) _ _ A _ _ _ pi1 pi2 _ _ _ _ _ _ _ eq_refl eq_refl);
-          try lia); clear IHf0.
-induction s as [s IHp0] using lt_wf_rect.
-assert (forall A B l1 l2 l3 l4 pi1 pi2, psize pi1 + psize pi2 < s -> fsize A <= c -> fsize B <= c ->
-          P A B l1 l2 l3 l4 pi1 pi2) as IHp
-  by (now intros A B l1 l2 l3 l4 pi1 pi2 Hp HA HB;
-          refine (IHp0 _ Hp _ _ _ _ pi1 pi2 _ _ _ _ _ _ _ eq_refl eq_refl)); clear IHp0.
-intros A B s1 s2 pi1 pi2 Heqs HA HB l1 l2 l3 l4 Heq1 Heq2; rewrite_all Heqs; clear s Heqs.
-destruct pi1.
-- destruct l1; inversion Heq1; subst; cbn in Heq1.
-  + destruct_eqrefl Heq1; apply Hax1.
-  + destruct l1; inversion Heq1; subst.
-    * destruct_eqrefl Heq1; apply Hax2.
-    * exfalso; destruct l1; inversion Heq1.
-- subst; cbn; apply Hex, IHp; cbn; rewrite ? psize_rew; lia.
-- destruct l1; inversion Heq1.
-  + destruct pi2; subst; cbn in HA; destruct_eqrefl Heq1.
-    * repeat (destruct l3; inversion Heq2); subst; destruct_eqrefl Heq2; apply Hsym;
-        [ apply Hax1 | apply Hax2 ].
-    * apply Hsym, Hex, IHp; cbn; rewrite ? psize_rew; lia.
-    * destruct l3; inversion Heq2; subst; cbn in HB.
-      -- destruct_eqrefl Heq2.
-         apply Htt; intros; apply IHf; lia.
-      -- apply Hsym.
-         dichot_elt_app_inf_exec H1; subst.
-         ++ replace (rew [ll] Heq2 in tens_r pi2_1 pi2_2)
-               with (rew <- (app_assoc (tens A1 B1 :: l3) _ _) in tens_r pi2_1 pi2_2).
-            ** apply Htens1, IHp; cbn; try lia.
-            ** rewrite <- (rew_opp_l ll (app_assoc (tens A1 B1 :: l3) (B :: l) l1)).
-               f_equal; rewrite rew_compose.
-               now assert (eq_trans Heq2 (app_assoc (tens A1 B1 :: l3) (B :: l) l1) = eq_refl)
-                     as -> by apply (Eqdep_dec.UIP_dec (@eq_dt_dec (list_dectype formulas_dectype)));
-                   cbn.
-         ++ replace (rew [ll] Heq2 in tens_r pi2_1 pi2_2)
-               with (rew (app_assoc (tens A1 B1 :: l6) _ _) in tens_r pi2_1 pi2_2).
-            ** apply Htens2, IHp; cbn; lia.
-            ** rewrite <- (rew_opp_r ll (app_assoc (tens A1 B1 :: l6) l2 (B :: l4))).
-               f_equal; unfold eq_rect_r; rewrite rew_compose.
-               now assert (eq_trans Heq2 (eq_sym (app_assoc (tens A1 B1 :: l6) l2 (B :: l4)))
-                         = eq_refl)
-                     as -> by apply (Eqdep_dec.UIP_dec (@eq_dt_dec (list_dectype formulas_dectype)));
-                   cbn.
-    * destruct l3; inversion Heq2; subst; destruct_eqrefl Heq2; cbn in HB.
-      -- apply Htp; intros; apply IHf; lia.
-      -- apply Hsym, Hparr, IHp; cbn; lia.
-  + subst; cbn.
-    dichot_elt_app_inf_exec H1; subst.
-    * change ((tens A0 B0 :: l1) ++ A :: l ++ l0) with (tens A0 B0 :: l1 ++ A :: l ++ l0) in Heq1.
-      replace (rew [ll] Heq1 in tens_r pi1_1 pi1_2)
-         with (rew <- (app_assoc (tens A0 B0 :: l1) _ _) in tens_r pi1_1 pi1_2).
-      -- apply Htens1, IHp; cbn; lia.
-      -- rewrite <- (rew_opp_l ll (app_assoc (tens A0 B0 :: l1) (A :: l) l0)).
-           f_equal; rewrite rew_compose.
-           now assert (eq_trans Heq1 (app_assoc (tens A0 B0 :: l1) (A :: l) l0) = eq_refl)
-                 as -> by apply (Eqdep_dec.UIP_dec (@eq_dt_dec (list_dectype formulas_dectype)));
-               cbn.
-    * change ((tens A0 B0 :: l5 ++ l6) ++ A :: l2)
-        with (tens A0 B0 :: (l5 ++ l6) ++ A :: l2) in Heq1.
-      replace (rew [ll] Heq1 in tens_r pi1_1 pi1_2)
-         with (rew (app_assoc (tens A0 B0 :: l5) _ _) in tens_r pi1_1 pi1_2).
-      -- apply Htens2, IHp; cbn; lia.
-      -- rewrite <- (rew_opp_r ll (app_assoc (tens A0 B0 :: l5) l6 (A :: l2))).
-         f_equal; unfold eq_rect_r; rewrite rew_compose.
-         now assert (eq_trans Heq1 (eq_sym (app_assoc (tens A0 B0 :: l5) l6 (A :: l2))) = eq_refl)
-               as -> by apply (Eqdep_dec.UIP_dec (@eq_dt_dec (list_dectype formulas_dectype)));
-             cbn.
-- destruct l1; inversion Heq1.
-  + destruct pi2; subst; cbn in HA; destruct_eqrefl Heq1.
-    * repeat (destruct l3; inversion Heq2); subst; destruct_eqrefl Heq2; apply Hsym;
-        [ apply Hax1 | apply Hax2 ].
-    * apply Hsym, Hex, IHp; cbn; rewrite ? psize_rew; lia.
-    * destruct l3; inversion Heq2; subst; cbn in HB.
-      -- destruct_eqrefl Heq2.
-         apply Hsym, Htp; intros; apply IHf; lia.
-      -- apply Hsym; cbn.
-         dichot_elt_app_inf_exec H1; subst.
-         ++ change ((tens A1 B1 :: l3) ++ B :: l ++ l1)
-              with (tens A1 B1 :: l3 ++ B :: l ++ l1) in Heq2.
-            replace (rew [ll] Heq2 in tens_r pi2_1 pi2_2)
-               with (rew <- (app_assoc (tens A1 B1 :: l3) _ _) in tens_r pi2_1 pi2_2).
-            ** apply Htens1, IHp; cbn; lia.
-            ** rewrite <- (rew_opp_l ll (app_assoc (tens A1 B1 :: l3) (B :: l) l1)).
-               f_equal; rewrite rew_compose.
-               now assert (eq_trans Heq2 (app_assoc (tens A1 B1 :: l3) (B :: l) l1) = eq_refl)
-                     as -> by apply (Eqdep_dec.UIP_dec (@eq_dt_dec (list_dectype formulas_dectype)));
-                   cbn.
-         ++ change ((tens A1 B1 :: l0 ++ l5) ++ B :: l4)
-              with (tens A1 B1 :: (l0 ++ l5) ++ B :: l4) in Heq2.
-            replace (rew [ll] Heq2 in tens_r pi2_1 pi2_2)
-               with (rew (app_assoc (tens A1 B1 :: l0) _ _) in tens_r pi2_1 pi2_2).
-            ** apply Htens2, IHp; cbn; lia.
-            ** rewrite <- (rew_opp_r ll (app_assoc (tens A1 B1 :: l0) l5 (B :: l4))).
-               f_equal; unfold eq_rect_r; rewrite rew_compose.
-               now assert (eq_trans Heq2 (eq_sym (app_assoc (tens A1 B1 :: l0) l5 (B :: l4)))
-                         = eq_refl)
-                     as -> by apply (Eqdep_dec.UIP_dec (@eq_dt_dec (list_dectype formulas_dectype)));
-                   cbn.
-    * destruct l3; inversion Heq2; subst; cbn in HB; destruct_eqrefl Heq2.
-      -- apply Hpp; intros; apply IHf; lia.
-      -- apply Hsym, Hparr, IHp; cbn; lia.
-  + subst; cbn; destruct_eqrefl Heq1.
-    apply Hparr, IHp; cbn; lia.
-Qed.
-
-Theorem cut A l1 l2 l3 l4 :
-  ll (l1 ++ A :: l2) -> ll (l3 ++ dual A :: l4) -> ll (l3 ++ l2 ++ l1 ++ l4).
-Proof.
-intros pi1 pi2; assert (Heq := eq_refl (dual A)); revert pi1 pi2 Heq.
-apply (sym_induction_ll (fun A B l1 l2 l3 l4 pi1 pi2 => B = dual A -> ll (l3 ++ l2 ++ l1 ++ l4)));
-  clear A l1 l2 l3 l4; cbn; try now intuition subst.
-- intros A B l1 l2 l3 l4 pi1 pi2 pi ->.
-  apply (ex_r (pi (eq_sym (bidual A)))).
-  rewrite (app_assoc l1), (app_assoc l3); apply Permutation_Type_app_comm.
-- intros A B l1 l2 l3 l4 l' pi1 pi2 HP.
-  destruct (Permutation_Type_vs_elt_inv A l1 l2 HP) as [(l1', l2') ->]; cbn in pi1, HP; cbn.
-  intros pi0' pi0; apply pi0' in pi0; clear - HP pi0.
-  apply (ex_r pi0).
-  apply Permutation_Type_app_head; rewrite ? app_assoc; apply Permutation_Type_app_tail.
-  transitivity (l1' ++ l2'); [ apply Permutation_Type_app_comm | ].
-  transitivity (l1 ++ l2); [ | apply Permutation_Type_app_comm ].
-  apply (Permutation_Type_app_inv _ _ _ _ _ HP).
-- intros A B C D l0 l1 l2 l3 l4 pi1 pi2 pi3 pi4 ->.
-  change (ll (l3 ++ (l2 ++ l0) ++ tens C D :: l1 ++ l4)).
-  apply ex_r with (tens C D :: ((l1 ++ l4) ++ l3 ++ l2) ++ l0); [ apply tens_r; trivial | ].
-  + apply (ex_r (pi4 eq_refl)).
-    rewrite app_assoc; apply Permutation_Type_app_comm.
-  + list_simpl; rewrite app_comm_cons, app_assoc, ? (app_assoc l3), (app_assoc (l3 ++ l2)).
-    apply Permutation_Type_app_comm.
-- intros A B C D l0 l1 l2 l3 l4 pi1 pi2 pi3 pi4' pi4; apply pi4' in pi4; clear pi4'.
-  apply ex_r with (tens C D :: l0 ++ (l1 ++ l4) ++ l3 ++ l2); [ apply tens_r; trivial | ].
-  + apply (ex_r pi4).
-    rewrite app_assoc; apply Permutation_Type_app_comm.
-  + list_simpl; rewrite app_comm_cons, ? (app_assoc l3), ? app_assoc, <- app_assoc.
-    apply Permutation_Type_app_comm.
-- intros A B C D l1 l2 l3 l4 pi1 pi2 pi3' pi3; apply pi3' in pi3; clear pi3'.
-  apply ex_r with (parr C D :: (l1 ++ l4) ++ l3 ++ l2); [ apply parr_r, (ex_r pi3) | ].
-  + rewrite app_assoc; apply Permutation_Type_app_comm.
-  + list_simpl; rewrite app_comm_cons, ? app_assoc, <- app_assoc.
-    apply Permutation_Type_app_comm.
-- intros C D C' D' l1 l2 pi1 pi2 IHC IHD l0 pi0 Heq; injection Heq as -> ->.
-  rewrite <- app_assoc; apply IHC; auto.
-  now rewrite <- app_nil_l; apply IHD.
-Qed.
 *)
-
 End Atoms.
